Refactoring all maps and sets proofs and lemmas + fix typo

theories/Map/MapLevelD.v
@@ -6,32 +6,30 @@ From DeBrLevel Require Import LevelInterface Level MapExtInterface MapExt MapLev
 (** * Implementation - Map - [OTK/LvlD] *)
 
 (** ** Leveled Map Implementation *)
-
-Module IsLvlMapD 
-  (Key : OrderedTypeWithLeibniz) (Data : IsLvlETWL) 
-  (M : Interface.S Key) (MO : MapInterface Key Data M) <: IsLvlMapDInterface Key Data M MO.
+Module IsLvlMapD (Key : OrderedTypeWithLeibniz) (Data : IsLvlETWL) (M : Interface.S Key) 
+                 (MO : MapInterface Key Data M) <: IsLvlMapDInterface Key Data M MO.
 
 Import MO OP.P.
 Include MO.            
 
-(** *** Definition *)
+(** *** Definitions *)
 
-Definition shift_func (lb k : Lvl.t) (key : M.key) (v : Data.t) (m : t) :=
-  M.add key (Data.shift lb k v) m.
+Definition shift_func (n k: Lvl.t) (key: M.key) (v: Data.t) (m: t) :=
+  M.add key (Data.shift n k v) m.
 
-Definition valid_func (lb : Lvl.t) (k : M.key) (v : Data.t) (P : Prop) :=
-  Data.valid lb v /\ P.
+Definition Wf_func (n: Lvl.t) (k: M.key) (v: Data.t) (P: Prop) := Data.Wf n v /\ P.
 
-Definition shift (lb k : Lvl.t) (m : t) := M.fold (shift_func lb k) m M.empty.
+Definition shift (n k: Lvl.t) (m: t) := M.fold (shift_func n k) m M.empty.
 
-Definition valid (lb : Lvl.t) (m : t) := M.fold (valid_func lb) m True.
+Definition Wf (n : Lvl.t) (m : t) := M.fold (Wf_func n) m True.
 
 (** *** Facts *)
 
 #[export] Instance iff_equiv : Equivalence iff := _.
+
 #[export] Instance logic_eq_equiv : forall A, Equivalence (@Logic.eq A) := _.
 
-Fact valid_diamond (lb : Lvl.t) : Diamond iff (valid_func lb).
+Fact Wf_func_diamond (n : Lvl.t) : Diamond iff (Wf_func n).
 Proof.
   unfold Diamond; intros; split; intros [bn iu].
   -- rewrite <- H1 in iu; destruct iu; split; auto.
@@ -40,10 +38,9 @@ Proof.
       rewrite <- H1; split; auto.
 Qed.
 
-#[export] Instance valid_proper :
-  Proper (Logic.eq ==> Key.eq ==> Logic.eq ==> iff ==> iff) valid_func.
+#[export] Instance Wf_func_iff : Proper (Logic.eq ==> Key.eq ==> Logic.eq ==> iff ==> iff) Wf_func.
 Proof. 
-  intros lb' lb HeqLvl k k' _ v' v HeqData P' P HeqP; subst.
+  intros n' n HeqLvl k k' _ v' v HeqData P' P HeqP; subst.
   split.
   - intros [Hv HP']; split; auto; now rewrite <- HeqP.
   - intros [Hv HP']; split; auto; now rewrite HeqP.
@@ -52,7 +49,7 @@ Qed.
 #[export] Instance shift_proper :
   Proper (Logic.eq ==> Logic.eq ==> Key.eq ==> Logic.eq ==> eq ==> eq) shift_func.
 Proof.
-  intros lb' lb Heqlb k' k Heqk key key' HeqKey v' v HeqData m m' Heqm y; subst.
+  intros n' n Heqlb k' k Heqk key key' HeqKey v' v HeqData m m' Heqm y; subst.
   unfold shift_func; rewrite Heqm.
   destruct (Key.eq_dec key y) as [Heqk | Hneqk].
   - repeat rewrite add_eq_o; auto.
@@ -61,7 +58,7 @@ Proof.
     now rewrite <- HeqKey.
 Qed.
 
-Fact shift_diamond (lb k : Lvl.t) : Diamond eq (shift_func lb k).
+Fact shift_diamond (n k : Lvl.t) : Diamond eq (shift_func n k).
 Proof.
   intros key key' v v' m m1 m2 HneqKey Heqm1 Heqm2. 
   rewrite <- Heqm1; rewrite <- Heqm2.
@@ -69,70 +66,70 @@ Proof.
   now rewrite add_add_2.
 Qed.
 
-
-(** *** extra [valid] property *)
-
-#[export] Hint Resolve iff_equiv Equal_equiv logic_eq_equiv valid_diamond valid_proper
+#[export] Hint Resolve iff_equiv Equal_equiv logic_eq_equiv Wf_func_diamond Wf_func_iff
                        shift_proper shift_diamond : core.
 
-Lemma valid_Empty_spec (lb : Lvl.t) (m : t) : Empty m -> valid lb m.
+(** *** Properties *)
+
+(** **** [Wf] properties *)
+
+Lemma Wf_Empty (n : Lvl.t) (m : t) : Empty m -> Wf n m.
 Proof.
-  intro HEmpty; unfold valid.
+  intro HEmpty; unfold Wf.
   rewrite fold_Empty with (m := m); eauto.
 Qed.
 
-Lemma valid_Empty_iff (lb : Lvl.t) (m : t) : Empty m -> valid lb m <-> True.
+Lemma Wf_Empty_iff (n : Lvl.t) (m : t) : Empty m -> Wf n m <-> True.
 Proof.
-  intro HEmpty; unfold valid.
+  intro HEmpty; unfold Wf.
   rewrite fold_Empty with (m := m); eauto.
   reflexivity.
 Qed.
 
-Lemma valid_empty_spec (lb : Lvl.t) : valid lb M.empty.
-Proof. apply valid_Empty_spec; apply empty_1. Qed.
+Lemma Wf_empty (n : Lvl.t) : Wf n M.empty.
+Proof. apply Wf_Empty; apply empty_1. Qed.
 
-Lemma valid_Add_iff (lb : Lvl.t) (x : Key.t) (v : Data.t) (m m' : t) :
-  ~ M.In x m -> Add x v m m' -> 
-  Data.valid lb v /\ valid lb m <-> valid lb m'.
+Lemma Wf_Add_iff (n : Lvl.t) (x : Key.t) (v : Data.t) (m m' : t) :
+  ~ M.In x m -> Add x v m m' -> Data.Wf n v /\ Wf n m <-> Wf n m'.
 Proof.
-  unfold valid, valid_func; intros HnIn HAdd.
+  unfold Wf, Wf_func; intros HnIn HAdd.
   symmetry.
   rewrite fold_Add with (i := True); eauto.
   - reflexivity.
-  - now apply valid_proper.
-  - now apply valid_diamond.
+  - now apply Wf_func_iff.
+  - now apply Wf_func_diamond.
 Qed.
   
-#[export] Instance valid_eq : Proper (Logic.eq ==> eq ==> iff) valid.
+#[export] Instance Wf_iff : Proper (Logic.eq ==> eq ==> iff) Wf.
 Proof.
-  intros lb' lb Heqlb m m' Heqm; subst.
+  intros n' n Heqlb m m' Heqm; subst.
   revert m' Heqm; induction m using map_induction; intros m' Heqm.
-  - repeat rewrite valid_Empty_iff; auto; try reflexivity.
+  - repeat rewrite Wf_Empty_iff; auto; try reflexivity.
     now rewrite <- Heqm.
-  - rewrite <- valid_Add_iff; eauto.
+  - rewrite <- Wf_Add_iff; eauto.
     symmetry.
-    rewrite <- valid_Add_iff with (v := e); eauto.
+    rewrite <- Wf_Add_iff with (v := e); eauto.
     -- reflexivity.
     -- unfold Add in *; now rewrite <- Heqm.
 Qed.
 
-Lemma valid_add_notin_spec (lb : Lvl.t) (x : Key.t) (v : Data.t) (m : t) :
-  ~ M.In x m -> valid lb (M.add x v m) <-> Data.valid lb v /\ valid lb m.
+Lemma Wf_add_notin (n : Lvl.t) (x : Key.t) (v : Data.t) (m : t) :
+  ~ M.In x m -> Wf n (M.add x v m) <-> Data.Wf n v /\ Wf n m.
 Proof.
   intros HnIn. 
-  rewrite (valid_Add_iff lb x v m (M.add x v m) HnIn).
+  rewrite (Wf_Add_iff n x v m (M.add x v m) HnIn).
   - reflexivity.
   - unfold Add; reflexivity.
 Qed.
 
-Lemma valid_add_in_spec (k : Lvl.t) (x : Key.t) (m : t) :
-  M.In x m -> valid k m -> exists v, valid k (M.add x v m).
+Lemma Wf_add_in (k : Lvl.t) (x : Key.t) (m : t) :
+  M.In x m -> Wf k m -> exists v, Wf k (M.add x v m).
 Proof.
   revert x; induction m using map_induction; intros y HIn Hv.
   - exfalso.
     destruct HIn as [v HMp].
     now apply (H y v).
-  - rewrite <- valid_Add_iff in Hv; eauto.
+  - rewrite <- Wf_Add_iff in Hv; eauto.
     destruct Hv as [Hve Hv].
     unfold Add in H0.
     destruct (Key.eq_dec y x) as [Heq | Hneq].
@@ -140,90 +137,90 @@ Proof.
        rewrite H0 in *.
        rewrite Heq.
        rewrite add_add_1.
-       rewrite valid_add_notin_spec; auto.
+       rewrite Wf_add_notin; auto.
     -- rewrite H0 in HIn.
        apply add_in_iff in HIn as [Heq | HIn]. 
        + symmetry in Heq; contradiction.
        + apply (IHm1 y HIn) in Hv as [v' Hv].
          exists v'.
          rewrite H0; rewrite add_add_2; auto.
-         apply valid_add_notin_spec; auto.
+         apply Wf_add_notin; auto.
          rewrite add_in_iff. 
          intros [c | c]; auto.
 Qed.
 
-Lemma valid_add_spec (lb : Lvl.t) (x : Key.t) (v : Data.t) (m : t) :
-  Data.valid lb v /\ valid lb m -> valid lb (M.add x v m).
+Lemma Wf_add (n : Lvl.t) (x : Key.t) (v : Data.t) (m : t) :
+  Data.Wf n v /\ Wf n m -> Wf n (M.add x v m).
 Proof.
   revert x v; induction m using map_induction; intros y v [Hv Hvm].
-  - apply Empty_eq_spec in H; rewrite H.
-    apply valid_add_notin_spec.
+  - apply Empty_eq in H; rewrite H.
+    apply Wf_add_notin.
     -- apply not_in_empty.
     -- split; auto.
-       apply valid_empty_spec.
+       apply Wf_empty.
   - unfold Add in H0; rewrite H0 in *; clear H0.
-    apply valid_add_notin_spec in Hvm as [Hve Hvm]; auto.
+    apply Wf_add_notin in Hvm as [Hve Hvm]; auto.
     destruct (Key.eq_dec y x) as [Heq | Hneq].
     -- rewrite Heq.
        rewrite add_shadow.
-       now apply valid_add_notin_spec.
+       now apply Wf_add_notin.
     -- rewrite add_add_2; auto. 
-       apply valid_add_notin_spec; auto.
+       apply Wf_add_notin; auto.
        rewrite add_in_iff.
        intros [c | c]; auto.
 Qed.
 
-Lemma valid_Add_spec (lb : Lvl.t) (x : Key.t) (v : Data.t) (m m' : t) :
+Lemma Wf_Add (n : Lvl.t) (x : Key.t) (v : Data.t) (m m' : t) :
   Add x v m m' -> 
-  Data.valid lb v /\ valid lb m -> valid lb m'.
+  Data.Wf n v /\ Wf n m -> Wf n m'.
 Proof. 
   intros HA Hv; unfold Add in HA.
   rewrite HA.
-  now apply valid_add_spec.
+  now apply Wf_add.
 Qed.
 
-Lemma valid_find_spec (lb : Lvl.t) (x : Key.t) (v : Data.t) (m : t) :
-  valid lb m -> M.find x m = Some v -> Data.valid lb v.
+Lemma Wf_find (n : Lvl.t) (x : Key.t) (v : Data.t) (m : t) :
+  Wf n m -> M.find x m = Some v -> Data.Wf n v.
 Proof.
   induction m using map_induction; intros Hv Hfi.
   - exfalso.
     apply find_2 in Hfi.
     now apply (H x v).
   - unfold Add in *; rewrite H0 in *; clear H0.
-    apply valid_add_notin_spec in Hv as [Hve Hvm1]; auto.
+    apply Wf_add_notin in Hv as [Hve Hvm1]; auto.
     rewrite add_o in Hfi.
     destruct (Key.eq_dec x0 x) as [Heq | Hneq]; auto.
     inversion Hfi; now subst.
 Qed. 
 
-Lemma valid_update_spec (lb : Lvl.t) (x : Key.t) (v : Data.t) (m : t) :
-  M.In x m -> valid lb m -> Data.valid lb v -> valid lb (M.add x v m).
+Lemma Wf_update (n : Lvl.t) (x : Key.t) (v : Data.t) (m : t) :
+  M.In x m -> Wf n m -> Data.Wf n v -> Wf n (M.add x v m).
 Proof.
   revert x v; induction m using map_induction; intros y v HIn Hvo Hvd.
-  - apply Empty_eq_spec in H; rewrite H in *.
+  - apply Empty_eq in H; rewrite H in *.
     inversion HIn.
     apply empty_mapsto_iff in H0; contradiction.
   - unfold Add in H0; rewrite H0 in *; clear H0.
-    apply valid_add_notin_spec in Hvo as [Hve Hvo1]; auto.
+    apply Wf_add_notin in Hvo as [Hve Hvo1]; auto.
     apply add_in_iff in HIn as [Heq | HIn]; subst.
     -- rewrite Heq in *. 
        rewrite add_shadow.
-       rewrite valid_add_notin_spec; auto.
+       rewrite Wf_add_notin; auto.
     -- destruct (Key.eq_dec y x) as [Heq| Hneq].
        + rewrite Heq in *. contradiction.
        + rewrite add_add_2; auto.
          eapply IHm1 in Hvo1; eauto.
-         rewrite valid_add_notin_spec; auto.
+         rewrite Wf_add_notin; auto.
          rewrite add_in_iff; intros [Hc | Hc]; subst; contradiction.
 Qed.
 
-(** *** extra [shift] property *)
+(** **** [shift] properties *)
 
 #[export] Instance shift_eq : Proper (Logic.eq ==> Logic.eq ==> eq ==> eq) shift.
 Proof.
-  intros lb' lb Heqlb k' k Heqk m; subst.
+  intros n' n Heqlb k' k Heqk m; subst.
   induction m using map_induction; intros m' Heqm; unfold shift.
-  - apply Empty_eq_spec in H as Heq.
+  - apply Empty_eq in H as Heq.
     repeat rewrite fold_Empty with (eqA := eq); auto.
     -- reflexivity.
     -- rewrite <- Heqm; rewrite Heq.
@@ -235,17 +232,17 @@ Proof.
     -- unfold Add in H0; now rewrite <- Heqm.
 Qed.
 
-Lemma shift_Empty_spec (lb k : Lvl.t) (m : t) :
-  Empty m -> eq (shift lb k m) m.
+Lemma shift_Empty (n k : Lvl.t) (m : t) :
+  Empty m -> eq (shift n k m) m.
 Proof. 
   intro HEmp; unfold shift.
   rewrite fold_Empty with (eqA := eq); eauto.
-  symmetry; now apply Empty_eq_spec.
+  symmetry; now apply Empty_eq.
 Qed.
 
-Lemma shift_add_notin_spec (lb k : Lvl.t) (x : Key.t) (v : Data.t) (m : t) :
+Lemma shift_add_notin (n k : Lvl.t) (x : Key.t) (v : Data.t) (m : t) :
   ~ M.In x m ->  
-  eq (shift lb k (M.add x v m)) (M.add x (Data.shift lb k v) (shift lb k m)).
+  eq (shift n k (M.add x v m)) (M.add x (Data.shift n k v) (shift n k m)).
 Proof.
   intro HnIn; unfold shift.
   rewrite fold_add with (eqA := eq) (i := M.empty); eauto.
@@ -253,8 +250,8 @@ Proof.
   - now apply shift_proper.
 Qed.
 
-Lemma shift_add_spec (lb k : Lvl.t) (x : Key.t) (v : Data.t) (m : t) :
-  eq (shift lb k (M.add x v m)) (M.add x (Data.shift lb k v) (shift lb k m)).
+Lemma shift_add (n k : Lvl.t) (x : Key.t) (v : Data.t) (m : t) :
+  eq (shift n k (M.add x v m)) (M.add x (Data.shift n k v) (shift n k m)).
 Proof.
   destruct (In_dec m x) as [HIn | HnIn].
   - revert HIn; induction m using map_induction; intro HIn.
@@ -265,42 +262,42 @@ Proof.
        apply add_in_iff in HIn as [Heq | HIn].
        + rewrite Heq in *; clear Heq.
          rewrite add_shadow.
-         repeat rewrite shift_add_notin_spec; auto.
+         repeat rewrite shift_add_notin; auto.
          now rewrite add_shadow.
        + destruct (Key.eq_dec x x0) as [Heq | Hneq].
          ++ rewrite Heq in *; clear Heq.
             contradiction.
          ++ apply IHm1 in HIn as Heq.
             rewrite add_add_2; auto.
-            rewrite shift_add_notin_spec.
+            rewrite shift_add_notin.
             * rewrite Heq.
-              rewrite shift_add_notin_spec; auto.
+              rewrite shift_add_notin; auto.
               rewrite add_add_2.
               ** reflexivity.
               ** intro c; symmetry in c.
                  contradiction.
             * rewrite add_in_iff.
               intros [c | c]; auto.
-  - now apply shift_add_notin_spec.
+  - now apply shift_add_notin.
 Qed.
 
-Lemma shift_Add_spec (lb k : Lvl.t) (key : Key.t) (v : Data.t) (m m' : t) :
+Lemma shift_Add (n k : Lvl.t) (key : Key.t) (v : Data.t) (m m' : t) :
   Add key v m m' -> 
-  eq (shift lb k m') (M.add key (Data.shift lb k v) (shift lb k m)).
+  eq (shift n k m') (M.add key (Data.shift n k v) (shift n k m)).
 Proof.
   unfold Add; intro HAdd.
   rewrite HAdd.
-  apply shift_add_spec.
+  apply shift_add.
 Qed.
   
-Lemma shift_in_spec_1 (lb k : Lvl.t) (key : Key.t) (m : t) :
-  M.In key m -> M.In key (shift lb k m).
+Lemma shift_in_1 (n k : Lvl.t) (key : Key.t) (m : t) :
+  M.In key m -> M.In key (shift n k m).
 Proof.
   induction m using map_induction; intro HIn.
   - exfalso.
     destruct HIn as [v HMp].
     now apply (H key v).
-  - apply shift_Add_spec with (lb := lb) (k := k) in H0 as H0'; auto.
+  - apply shift_Add with (n := n) (k := k) in H0 as H0'; auto.
     rewrite in_find in *. 
     rewrite H0',H0 in *. 
     rewrite <- in_find in *. 
@@ -308,34 +305,34 @@ Proof.
     destruct HIn; auto.
 Qed.
 
-Lemma shift_in_spec_2 (lb k : Lvl.t) (key : Key.t) (m : t) :
-  M.In key (shift lb k m) -> M.In key m.
+Lemma shift_in_2 (n k : Lvl.t) (key : Key.t) (m : t) :
+  M.In key (shift n k m) -> M.In key m.
 Proof.
   induction m using map_induction; intro HIn.
   - exfalso.
-    rewrite shift_Empty_spec in HIn; auto.
+    rewrite shift_Empty in HIn; auto.
     destruct HIn as [v HMp].
     now apply (H key v). 
-  - rewrite shift_Add_spec in HIn; eauto.
+  - rewrite shift_Add in HIn; eauto.
     unfold Add in *; rewrite H0; clear H0.
     rewrite add_in_iff in *.
     destruct HIn as [Heq | HIn]; auto.
 Qed.
 
-Lemma shift_in_iff (lb k : Lvl.t) (key : Key.t) (m : t) : 
-  M.In key m <-> M.In key (shift lb k m).
+Lemma shift_in_iff (n k : Lvl.t) (key : Key.t) (m : t) : 
+  M.In key m <-> M.In key (shift n k m).
 Proof.
   split; intro HIn.
-  - apply shift_in_spec_1; auto.
-  - eapply shift_in_spec_2; eauto. 
+  - apply shift_in_1; auto.
+  - eapply shift_in_2; eauto. 
 Qed.
 
-Lemma shift_notin_iff (lb k : Lvl.t) (key : Key.t) (m : t) : 
-  ~ M.In key m <-> ~ M.In key (shift lb k m).
+Lemma shift_notin_iff (n k : Lvl.t) (key : Key.t) (m : t) : 
+  ~ M.In key m <-> ~ M.In key (shift n k m).
 Proof. now rewrite <- shift_in_iff. Qed.
 
-Lemma shift_find_iff (lb k : Lvl.t) (key : Key.t) (v : Data.t) (m : t) : 
-  M.find key m = Some v <-> M.find key (shift lb k m) = Some (Data.shift lb k v).
+Lemma shift_find_iff (n k : Lvl.t) (key : Key.t) (v : Data.t) (m : t) : 
+  M.find key m = Some v <-> M.find key (shift n k m) = Some (Data.shift n k v).
 Proof.
   induction m using map_induction.
   - split; intro Hfi.
@@ -343,10 +340,10 @@ Proof.
        apply (H key v).
        now apply find_2.
     -- exfalso.
-       rewrite shift_Empty_spec in Hfi; auto.
-       apply (H key (Data.shift lb k v)).
+       rewrite shift_Empty in Hfi; auto.
+       apply (H key (Data.shift n k v)).
        now apply find_2.
-  - rewrite shift_Add_spec with (lb := lb) (k := k); eauto.
+  - rewrite shift_Add with (n := n) (k := k); eauto.
     unfold Add in H0; rewrite H0.
     destruct (Key.eq_dec x key).
     -- repeat rewrite add_eq_o; auto. 
@@ -362,20 +359,20 @@ Proof.
          now rewrite IHm1.
 Qed.
 
-Lemma shift_Empty_iff (lb k : Lvl.t) (m : t) :
-  Empty m <-> Empty (shift lb k m).
+Lemma shift_Empty_iff (n k : Lvl.t) (m : t) :
+  Empty m <-> Empty (shift n k m).
 Proof.
   split; intro HEmp.
-  - rewrite shift_Empty_spec; auto.
+  - rewrite shift_Empty; auto.
   - intros key v HMp.
-    apply (HEmp key (Data.shift lb k v)).
+    apply (HEmp key (Data.shift n k v)).
     apply find_2.
     apply shift_find_iff.
     now apply find_1. 
 Qed.
 
-Lemma shift_eq_iff (lb k : Lvl.t) (m m1 : t) : 
-  eq m m1 <-> eq (shift lb k m) (shift lb k m1).
+Lemma shift_eq_iff (n k : Lvl.t) (m m1 : t) : 
+  eq m m1 <-> eq (shift n k m) (shift n k m1).
 Proof.
   split; intro Heq.
   - now rewrite Heq.
@@ -397,89 +394,89 @@ Proof.
        + now apply not_in_find.
 Qed.
 
-Lemma shift_Add_iff (lb k : Lvl.t) (key : Key.t) (v : Data.t) (m m' : t) :
+Lemma shift_Add_iff (n k : Lvl.t) (key : Key.t) (v : Data.t) (m m' : t) :
   Add key v m m' <->
-  Add key (Data.shift lb k v) (shift lb k m) (shift lb k m').
+  Add key (Data.shift n k v) (shift n k m) (shift n k m').
 Proof.
   split.
-  - apply shift_Add_spec.
+  - apply shift_Add.
   - unfold Add; intro HAdd.
-    rewrite <- shift_add_spec in HAdd. 
+    rewrite <- shift_add in HAdd. 
     eapply shift_eq_iff; eauto.
 Qed.
 
-Lemma shift_remove_spec (lb k : Lvl.t) (x : Key.t) (t : t) :
-  eq (M.remove x (shift lb k t)) (shift lb k (M.remove x t)).
+Lemma shift_remove (n k : Lvl.t) (x : Key.t) (t : t) :
+  eq (M.remove x (shift n k t)) (shift n k (M.remove x t)).
 Proof.
   induction t using map_induction.
-  - repeat rewrite shift_Empty_spec; auto; try reflexivity.
+  - repeat rewrite shift_Empty; auto; try reflexivity.
     intros key v HMp.
     apply remove_3 in HMp.
     now apply (H key v).
   - unfold Add in H0; rewrite H0; clear H0. 
-    rewrite shift_add_notin_spec; auto.
+    rewrite shift_add_notin; auto.
     destruct (Key.eq_dec x0 x) as [Heq | Hneq].
     -- rewrite <- Heq in *. 
        now repeat rewrite remove_add_1.
     -- repeat rewrite remove_add_2; auto.
        rewrite IHt1.
-       rewrite shift_add_notin_spec; auto; try reflexivity.
+       rewrite shift_add_notin; auto; try reflexivity.
        intros [v HMp].
        apply remove_3 in HMp.
        apply H; now exists v.
 Qed.
 
-Lemma shift_zero_refl (lb : Lvl.t) (t : t) : eq (shift lb 0 t) t.
+Lemma shift_zero_refl (n : Lvl.t) (t : t) : eq (shift n 0 t) t.
 Proof.
   induction t using map_induction.
-  - now apply shift_Empty_spec.
+  - now apply shift_Empty.
   - unfold Add in H0; rewrite H0 in *; clear H0.
-    rewrite shift_add_notin_spec; auto.
+    rewrite shift_add_notin; auto.
     rewrite IHt1.
-    assert (HeqD : (Data.shift lb 0 e) = e).
+    assert (HeqD : (Data.shift n 0 e) = e).
     { apply Data.eq_leibniz; now apply Data.shift_zero_refl. }
     now rewrite HeqD.
 Qed.
 
-Lemma shift_trans (lb k k' : Lvl.t) (t : t) :
-  eq (shift lb k (shift lb k' t)) (shift lb (k + k') t).
+Lemma shift_trans (n k k' : Lvl.t) (t : t) :
+  eq (shift n k (shift n k' t)) (shift n (k + k') t).
 Proof.
   induction t using map_induction. 
-  - repeat rewrite shift_Empty_spec; auto; reflexivity.
+  - repeat rewrite shift_Empty; auto; reflexivity.
   - unfold Add in H0; rewrite H0; clear H0.
-    repeat rewrite shift_add_notin_spec; auto.
-    -- replace (Data.shift lb (k + k') e) 
-       with (Data.shift lb k (Data.shift lb k' e)).
+    repeat rewrite shift_add_notin; auto.
+    -- replace (Data.shift n (k + k') e) 
+       with (Data.shift n k (Data.shift n k' e)).
        + now rewrite IHt1.
        + apply Data.eq_leibniz. 
          now apply Data.shift_trans.
     -- now rewrite <- shift_notin_iff.
 Qed.
 
-Lemma shift_permute (lb k k' : Lvl.t) (t : t) :
-  eq (shift lb k (shift lb k' t)) (shift lb k' (shift lb k t)).
+Lemma shift_permute (n k k' : Lvl.t) (t : t) :
+  eq (shift n k (shift n k' t)) (shift n k' (shift n k t)).
 Proof.
   induction t using map_induction.
-  - repeat rewrite shift_Empty_spec; auto; reflexivity.
+  - repeat rewrite shift_Empty; auto; reflexivity.
   - unfold Add in H0; rewrite H0; clear H0.
-    repeat rewrite shift_add_notin_spec; auto.
-    -- replace (Data.shift lb k' (Data.shift lb k e)) 
-       with (Data.shift lb k (Data.shift lb k' e)).
+    repeat rewrite shift_add_notin; auto.
+    -- replace (Data.shift n k' (Data.shift n k e)) 
+       with (Data.shift n k (Data.shift n k' e)).
        + now rewrite IHt1.
        + apply Data.eq_leibniz; apply Data.shift_permute.
     -- now rewrite <- shift_notin_iff.
     -- now rewrite <- shift_notin_iff.
 Qed.
 
-Lemma shift_unfold (lb k k' : Lvl.t) (t : t) :
-  eq (shift lb (k + k') t) (shift (lb + k) k' (shift lb k t)). 
+Lemma shift_unfold (n k k' : Lvl.t) (t : t) :
+  eq (shift n (k + k') t) (shift (n + k) k' (shift n k t)). 
 Proof.
   induction t using map_induction.
-  - repeat rewrite shift_Empty_spec; auto; reflexivity.
+  - repeat rewrite shift_Empty; auto; reflexivity.
   - unfold Add in H0; rewrite H0; clear H0.
-    repeat rewrite shift_add_notin_spec; auto.
-    -- replace (Data.shift (lb + k) k' (Data.shift lb k e)) 
-       with (Data.shift lb (k + k') e).
+    repeat rewrite shift_add_notin; auto.
+    -- replace (Data.shift (n + k) k' (Data.shift n k e)) 
+       with (Data.shift n (k + k') e).
        + now rewrite IHt1.
        + apply Data.eq_leibniz. apply Data.shift_unfold.
     -- now rewrite <- shift_notin_iff.  
@@ -490,9 +487,9 @@ Lemma shift_unfold_1 (k k' k'' : Lvl.t) (t : t) :
   eq (shift k' (k'' - k') (shift k  (k' - k) t)) (shift k (k'' - k) t).
 Proof.
   intros Hlt Hlt'; induction t using map_induction.
-  - repeat rewrite shift_Empty_spec; auto; reflexivity. 
+  - repeat rewrite shift_Empty; auto; reflexivity. 
   - unfold Add in H0; rewrite H0; clear H0.
-    repeat rewrite shift_add_notin_spec; auto.
+    repeat rewrite shift_add_notin; auto.
     -- replace (Data.shift k' (k'' - k') (Data.shift k (k' - k) e))
        with (Data.shift k (k'' - k) e).
        + now rewrite IHt1.
@@ -500,83 +497,83 @@ Proof.
     -- now rewrite <- shift_in_iff.
 Qed.
 
+(** **** Interaction properties between [Wf] and [shift] *)
 
-(** *** Interaction property between [valid] and [shift]  *)
-
-
-Lemma valid_weakening (k k' : Lvl.t) (t : t) : (k <= k') -> valid k t -> valid k' t.
+Lemma Wf_weakening (k k' : Lvl.t) (t : t) : (k <= k') -> Wf k t -> Wf k' t.
 Proof.
   induction t using map_induction; intros Hle Hvt.
-  - apply (valid_Empty_spec k' t0 H).
-  - rewrite <- valid_Add_iff; eauto.
-    rewrite <- valid_Add_iff in Hvt; eauto.
+  - apply (Wf_Empty k' t0 H).
+  - rewrite <- Wf_Add_iff; eauto.
+    rewrite <- Wf_Add_iff in Hvt; eauto.
     destruct Hvt as [Hv Hvt1]; split. 
-    -- now apply Data.valid_weakening with k.
+    -- now apply Data.Wf_weakening with k.
     -- now apply IHt1.
 Qed.
 
-Lemma shift_preserves_valid_1 (lb k k' : Lvl.t) (t : t) : 
-  valid k t -> valid (k + k') (shift lb k' t).
+Lemma shift_preserves_wf_1 (n k k' : Lvl.t) (t : t) : 
+  Wf k t -> Wf (k + k') (shift n k' t).
 Proof.
   induction t using map_induction; intro Hvt.
-  - rewrite shift_Empty_spec; auto.
-    apply (valid_Empty_spec _ t0 H).
+  - rewrite shift_Empty; auto.
+    apply (Wf_Empty _ t0 H).
   - unfold Add in H0; rewrite H0 in *; clear H0. 
-    rewrite shift_add_notin_spec; auto.
-    rewrite valid_add_notin_spec in *; auto.
+    rewrite shift_add_notin; auto.
+    rewrite Wf_add_notin in *; auto.
     -- destruct Hvt as [Hve Hvt1].
        split; auto.
-       now apply Data.shift_preserves_valid_1.
+       now apply Data.shift_preserves_wf_1.
     -- now apply shift_notin_iff.
 Qed.
 
-Lemma shift_preserves_valid_gen (lb lb' k k' : Lvl.t) (t : t) :
-  k <= k' -> lb <= lb' -> k <= lb -> k' <= lb' -> k' - k = lb' - lb -> 
-  valid lb t -> valid lb' (shift k (k' - k) t).
+Lemma shift_preserves_wf_gen (n p k m : Lvl.t) (t : t) :
+  k <= m -> n <= p -> k <= n -> m <= p -> m - k = p - n -> 
+  Wf n t -> Wf p (shift k (m - k) t).
 Proof.
   induction t using map_induction; intros Hle Hle1 Hle2 Hle3 Heq Hvt.
-  - rewrite shift_Empty_spec; auto.
-    apply (valid_Empty_spec _ _ H).
+  - rewrite shift_Empty; auto.
+    apply (Wf_Empty _ _ H).
   - unfold Add in H0; rewrite H0 in *; clear H0.
-    apply valid_add_notin_spec in Hvt as [Hve Hvt1]; auto.
-    rewrite shift_add_notin_spec; auto.
-    apply valid_add_notin_spec.
+    apply Wf_add_notin in Hvt as [Hve Hvt1]; auto.
+    rewrite shift_add_notin; auto.
+    apply Wf_add_notin.
     -- now apply shift_notin_iff.
     -- split; auto.
-       now apply Data.shift_preserves_valid_gen with (lb := lb).
+       now apply Data.shift_preserves_wf_gen with (m := n).
 Qed.
 
-Lemma shift_preserves_valid_2 (lb lb' : Lvl.t) (t : t) :
-lb <= lb' -> valid lb t -> valid lb' (shift lb (lb' - lb) t).
-Proof. intros; eapply shift_preserves_valid_gen; eauto. Qed.
+Lemma shift_preserves_wf_2 (n p : Lvl.t) (t : t) :
+n <= p -> Wf n t -> Wf p (shift n (p - n) t).
+Proof. intros; eapply shift_preserves_wf_gen; eauto. Qed.
 
-Lemma shift_preserves_valid (k k' : Lvl.t) (t : t) : 
-  valid k t -> valid (k + k') (shift k k' t).
-Proof. intros; now apply shift_preserves_valid_1. Qed.
+Lemma shift_preserves_wf (k m : Lvl.t) (t : t) : 
+  Wf k t -> Wf (k + m) (shift k m t).
+Proof. intros; now apply shift_preserves_wf_1. Qed.
 
-Lemma shift_preserves_valid_zero (k : Lvl.t) (t : t) : 
-  valid k t -> valid k (shift k 0 t).
-Proof. intros; replace k with (k + 0) by lia; now apply shift_preserves_valid_1. Qed.
+Lemma shift_preserves_wf_zero (k : Lvl.t) (t : t) : 
+  Wf k t -> Wf k (shift k 0 t).
+Proof. intros; replace k with (k + 0) by lia; now apply shift_preserves_wf_1. Qed.
 
 End IsLvlMapD.
 
 
+(** ---- *)
+
+
 (** ** Bindless Leveled Map Implementation *)
-Module IsBdlLvlMapD  
-  (Key : OrderedTypeWithLeibniz) (Data : IsBdlLvlETWL) 
-  (M : Interface.S Key) (MO : MapInterface Key Data M) <: IsBdlLvlMapDInterface Key Data M MO.
+Module IsBdlLvlMapD (Key : OrderedTypeWithLeibniz) (Data : IsBdlLvlETWL) (M : Interface.S Key) 
+                    (MO : MapInterface Key Data M) <: IsBdlLvlMapDInterface Key Data M MO.
 
 Include IsLvlMapD Key Data M MO.
 Import MO OP.P.  
 
-Lemma shift_valid_refl (lb k : Lvl.t) (t : t) : valid lb t -> eq (shift lb k t) t.
+Lemma shift_wf_refl (n k : Lvl.t) (t : t) : Wf n t -> eq (shift n k t) t.
 Proof.
   induction t using map_induction; intro Hvt.
-  - now apply shift_Empty_spec.
+  - now apply shift_Empty.
   - unfold Add in H0; rewrite H0 in *; clear H0. 
-    rewrite shift_add_notin_spec; auto. 
-    apply valid_add_notin_spec in Hvt as [Hv Hv']; auto.
-    eapply Data.shift_valid_refl in Hv; auto. 
+    rewrite shift_add_notin; auto. 
+    apply Wf_add_notin in Hvt as [Hv Hv']; auto.
+    eapply Data.shift_wf_refl in Hv; auto. 
     apply Data.eq_leibniz in Hv. 
     rewrite Hv.
     now rewrite IHt1.
@@ -584,26 +581,25 @@ Qed.
 
 End IsBdlLvlMapD.
 
+
 (** ---- *)
 
-(** * Make - Leveled Map [OTK/LvlD] *)
 
-Module MakeLvlMapD 
-  (Key : OrderedTypeWithLeibniz) (Data : IsLvlETWL) <: IsLvlET.
+(** * Make - Leveled Map [OTK/LvlD] *)
+Module MakeLvlMapD (Key : OrderedTypeWithLeibniz) (Data : IsLvlETWL) <: IsLvlET.
   
-  Module Raw := MMaps.OrdList.Make Key.
-  Module Ext := MapET Key Data Raw.
-  Include IsLvlMapD Key Data Raw Ext.
-  Include OP.P.
+Module Raw := MMaps.OrdList.Make Key.
+Module Ext := MapET Key Data Raw.
+Include IsLvlMapD Key Data Raw Ext.
+Include OP.P.
 
 End MakeLvlMapD.
 
-Module MakeBdlLvlMapD 
-  (Key : OrderedTypeWithLeibniz) (Data : IsBdlLvlETWL) <: IsBdlLvlET.
-  
-  Module Raw := MMaps.OrdList.Make Key.
-  Module Ext := MapET Key Data Raw.
-  Include IsBdlLvlMapD Key Data Raw Ext.
-  Include OP.P.
+Module MakeBdlLvlMapD (Key : OrderedTypeWithLeibniz) (Data : IsBdlLvlETWL) <: IsBdlLvlET.
+
+Module Raw := MMaps.OrdList.Make Key.
+Module Ext := MapET Key Data Raw.
+Include IsBdlLvlMapD Key Data Raw Ext.
+Include OP.P.
 
 End MakeBdlLvlMapD.
