theories/Map/MapLevelKD.v
@@ -5,32 +5,31 @@ From MMaps Require Import MMaps.
 (** * Implementation - Map - [LvlK/LvlD] *)
 
 (** ** Leveled Map Implementation *)
-Module IsLvlMapKD  
-  (Key : IsLvlOTWL) (Data : IsLvlETWL) 
-  (M : Interface.S Key) (MO : MapInterface Key Data M) <: IsLvlMapKDInterface Key Data M MO.
+Module IsLvlMapKD (Key : IsLvlOTWL) (Data : IsLvlETWL) (M : Interface.S Key) 
+                  (MO : MapInterface Key Data M) <: IsLvlMapKDInterface Key Data M MO.
 
 Import MO OP.P.
 Include MO.
 
-(** *** Definition *)
+(** *** Definitions *)
 
-Definition shift_func (lb k : Lvl.t) (key : Key.t) (v : Data.t) (m : t) :=
+Definition shift_func (lb k: Lvl.t) (key: Key.t) (v: Data.t) (m: t) :=
   M.add (Key.shift lb k key) (Data.shift lb k v) m.
 
-Definition valid_func (lb : Lvl.t) (key : Key.t) (v : Data.t) (P : Prop) :=
-  (Key.valid lb key) /\ (Data.valid lb v) /\ P.
+Definition Wf_func (lb: Lvl.t) (key: Key.t) (v: Data.t) (P: Prop) :=
+ (Key.Wf lb key) /\ (Data.Wf lb v) /\ P.
 
-Definition shift (lb k : Lvl.t) (m : t) := M.fold (shift_func lb k) m M.empty.
+Definition shift (lb k: Lvl.t) (m: t) := M.fold (shift_func lb k) m M.empty.
 
-Definition valid (lb : Lvl.t) (m : t) := M.fold (valid_func lb) m True.
-
+Definition Wf (lb: Lvl.t) (m: t) := M.fold (Wf_func lb) m True.
 
 (** *** Facts *)
 
 #[export] Instance iff_equiv : Equivalence iff := _.
+
 #[export] Instance logic_eq_equiv : forall A, Equivalence (@Logic.eq A) := _.
 
-Fact valid_diamond (lb : Lvl.t) : Diamond iff (valid_func lb).
+Fact Wf_func_diamond (lb: Lvl.t) : Diamond iff (Wf_func lb).
 Proof.
   intros k k' v v' P P' P'' HneqK HvfP HvfP'.
   split; intros [HvK [HvD HvP]].
@@ -46,18 +45,17 @@ Proof.
     now repeat split.
 Qed.
 
-#[export] Instance valid_proper : 
-  Proper (Logic.eq ==> Key.eq ==> Logic.eq ==> iff ==> iff) valid_func.
+#[export] Instance Wf_func_iff : Proper (Logic.eq ==> Key.eq ==> Logic.eq ==> iff ==> iff) Wf_func.
 Proof.
   intros lb' lb Heqlb k' k HeqK v' v HeqD P P' HeqP; subst.
   split; intros [Hvk [Hvd HvP]]. 
   - repeat split; auto.
-    -- eapply Key.valid_eq; eauto. 
+    -- eapply Key.Wf_iff; eauto. 
        + reflexivity.
        + now rewrite HeqK.
     -- now rewrite <- HeqP.
   - repeat split; auto.
-    -- eapply Key.valid_eq; eauto; reflexivity. 
+    -- eapply Key.Wf_iff; eauto; reflexivity. 
     -- now rewrite HeqP.
 Qed.
 
@@ -70,7 +68,7 @@ Proof.
   now apply Key.eq_leibniz in HeqK; subst. 
 Qed.
 
-Fact shift_diamond (lb k : Lvl.t) : Diamond eq (shift_func lb k).
+Fact shift_diamond (lb k: Lvl.t) : Diamond eq (shift_func lb k).
 Proof.
   intros ke ke' v v' P P' P'' HneqK Heq1 Heq2.
   unfold shift_func in *.
@@ -79,133 +77,130 @@ Proof.
   now rewrite <- Key.shift_eq_iff.
 Qed.
 
-
-(** *** extra [valid] property *)
-
-#[local] Hint Resolve iff_equiv Equal_equiv logic_eq_equiv valid_diamond valid_proper
+#[local] Hint Resolve iff_equiv Equal_equiv logic_eq_equiv Wf_func_diamond Wf_func_iff
 shift_proper shift_diamond : core.
 
-Lemma valid_Empty_spec (lb : Lvl.t) (m : t) : Empty m -> valid lb m.
+(** *** extra [Wf] properties *)
+
+Lemma Wf_Empty (lb: Lvl.t) (m: t) : Empty m -> Wf lb m.
 Proof.
-  intro HEmp; unfold valid.
+  intro HEmp; unfold Wf.
   rewrite fold_Empty; auto.
 Qed.
 
-Lemma valid_Empty_iff (lb : Lvl.t) (m : t) : Empty m -> valid lb m <-> True.
+Lemma Wf_Empty_iff (lb: Lvl.t) (m: t) : Empty m -> Wf lb m <-> True.
 Proof.
-  intro HEmp; unfold valid.
+  intro HEmp; unfold Wf.
   rewrite fold_Empty; auto; reflexivity.
 Qed.
 
-Lemma valid_empty_spec (lb : Lvl.t) : valid lb M.empty.
+Lemma Wf_empty (lb: Lvl.t) : Wf lb M.empty.
 Proof.
-  unfold valid; rewrite fold_Empty; auto.
+  unfold Wf; rewrite fold_Empty; auto.
   apply empty_1.
 Qed.
 
-Lemma valid_add_notin_spec (lb : Lvl.t) (x : Key.t) (v : Data.t) (m : t) :
+Lemma Wf_add_notin (lb: Lvl.t) (x: Key.t) (v: Data.t) (m: t) :
   ~ M.In x m -> 
-  valid lb (M.add x v m) <-> Key.valid lb x /\ Data.valid lb v /\ valid lb m.
+  Wf lb (M.add x v m) <-> Key.Wf lb x /\ Data.Wf lb v /\ Wf lb m.
 Proof.
-  unfold valid in *; intro HnIn.
+  unfold Wf in *; intro HnIn.
   rewrite fold_add; auto.
   - reflexivity.
-  - now apply valid_proper.
+  - now apply Wf_func_iff.
 Qed.
 
-Lemma valid_Add_iff (lb : Lvl.t) (x : Key.t) (v : Data.t) (m m' : t) :
+Lemma Wf_Add_iff (lb: Lvl.t) (x: Key.t) (v: Data.t) (m m': t) :
   ~ M.In x m -> Add x v m m' -> 
-  Key.valid lb x /\ Data.valid lb v /\ valid lb m <-> valid lb m'.
+  Key.Wf lb x /\ Data.Wf lb v /\ Wf lb m <-> Wf lb m'.
 Proof.
-  unfold valid in *; split; intros.
+  unfold Wf in *; split; intros.
   - rewrite fold_Add with (i := True); eauto.
-    now apply valid_proper.
+    now apply Wf_func_iff.
   - rewrite fold_Add with (i := True) in H1; eauto.
-    now apply valid_proper.
+    now apply Wf_func_iff.
 Qed.
 
-#[export] Instance valid_eq : Proper (Logic.eq ==> eq ==> iff) valid.
+#[export] Instance Wf_iff : Proper (Logic.eq ==> eq ==> iff) Wf.
 Proof.
   intros lb' lb Heqlb m m' Heqm; subst.
   revert m' Heqm; induction m using map_induction; intros m' Heqm.
   - split; intro Hvm.
-    -- apply valid_Empty_spec. 
+    -- apply Wf_Empty. 
        now rewrite <- Heqm.
-    -- now apply valid_Empty_spec. 
+    -- now apply Wf_Empty. 
   - split; intro Hvm.
-    -- rewrite <- valid_Add_iff in Hvm; eauto.
+    -- rewrite <- Wf_Add_iff in Hvm; eauto.
        destruct Hvm as [Hvx [Hve Hvm]].
-       rewrite <- valid_Add_iff; eauto.
+       rewrite <- Wf_Add_iff; eauto.
        unfold Add in *; now rewrite H0 in *.
-    -- rewrite <- valid_Add_iff with (v := e) in Hvm; eauto.
+    -- rewrite <- Wf_Add_iff with (v := e) in Hvm; eauto.
        + destruct Hvm as [Hvx [Hve Hvm]].
-         rewrite <- valid_Add_iff; eauto.
+         rewrite <- Wf_Add_iff; eauto.
        + unfold Add in *; now rewrite H0 in *.
 Qed.
 
-Lemma valid_add_spec (lb : Lvl.t) (x : Key.t) (v : Data.t) (m : t) :
-  Key.valid lb x /\ Data.valid lb v /\ valid lb m -> valid lb (M.add x v m).
+Lemma Wf_add (lb: Lvl.t) (x: Key.t) (v: Data.t) (m: t) :
+  Key.Wf lb x /\ Data.Wf lb v /\ Wf lb m -> Wf lb (M.add x v m).
 Proof.
   induction m using map_induction; intros [HvK [HvD Hvm]].
-  - rewrite valid_add_notin_spec; auto.
-    rewrite Empty_eq_spec; auto.
+  - rewrite Wf_add_notin; auto.
+    rewrite Empty_eq; auto.
     apply not_in_empty.
   - unfold Add in *; rewrite H0 in *; clear H0. 
-    apply valid_add_notin_spec in Hvm as [Hvx0 [Hve Hvm]]; auto.
+    apply Wf_add_notin in Hvm as [Hvx0 [Hve Hvm]]; auto.
     destruct (Key.eq_dec x x0) as [Heq | Hneq].
     -- rewrite Heq in *.
        rewrite add_shadow.
-       now apply valid_add_notin_spec.
+       now apply Wf_add_notin.
     -- rewrite add_add_2; auto.
-       apply valid_add_notin_spec.
+       apply Wf_add_notin.
        + rewrite add_in_iff.
          intros [Heq | HIn]; auto.
        + repeat split; auto.
 Qed.
 
-Lemma valid_find_spec (lb : Lvl.t) (x : Key.t) (v : Data.t) (m : t) :
-  valid lb m -> M.find x m = Some v -> Key.valid lb x /\ Data.valid lb v.
+Lemma Wf_find (lb: Lvl.t) (x: Key.t) (v: Data.t) (m: t) :
+  Wf lb m -> M.find x m = Some v -> Key.Wf lb x /\ Data.Wf lb v.
 Proof.
   induction m using map_induction; intros Hvm Hfm.
-  - rewrite Empty_eq_spec in Hfm; auto.
+  - rewrite Empty_eq in Hfm; auto.
     rewrite empty_o in Hfm.
     inversion Hfm.
   - unfold Add in *; rewrite H0 in *; clear H0.
-    apply valid_add_notin_spec in Hvm as [Hvx0 [Hve Hvm]]; auto.
+    apply Wf_add_notin in Hvm as [Hvx0 [Hve Hvm]]; auto.
     destruct (Key.eq_dec x0 x) as [Heq | Hneq].
     -- rewrite add_eq_o in Hfm; auto.
        inversion Hfm; subst; clear Hfm.
        split; auto.
-       eapply Key.valid_eq; eauto; try reflexivity.
+       eapply Key.Wf_iff; eauto; try reflexivity.
        now symmetry.
     -- rewrite add_neq_o in Hfm; auto.
 Qed. 
 
-Lemma valid_in_spec (lb : Lvl.t) (x : Key.t) (m : t) :
-  valid lb m -> M.In x m -> Key.valid lb x.
+Lemma Wf_in (lb: Lvl.t) (x: Key.t) (m: t) : Wf lb m -> M.In x m -> Key.Wf lb x.
 Proof.
   intros Hvm [v Hfm].
   apply find_1 in Hfm.
-  now apply (valid_find_spec lb x v m Hvm) in Hfm as [Hvx _].
+  now apply (Wf_find lb x v m Hvm) in Hfm as [Hvx _].
 Qed. 
 
-Lemma valid_add_in_spec (lb : Lvl.t) (x : Key.t) (m : t) :
-  M.In x m -> valid lb m -> exists v, valid lb (M.add x v m).
+Lemma Wf_add_in (lb: Lvl.t) (x: Key.t) (m: t) : M.In x m -> Wf lb m -> exists v, Wf lb (M.add x v m).
 Proof.
   induction m using map_induction; intros HIn Hvm.
   - exfalso.
-    rewrite Empty_eq_spec in HIn; auto.
+    rewrite Empty_eq in HIn; auto.
     now apply not_in_empty in HIn.
-  - rewrite <- valid_Add_iff in Hvm; eauto.
+  - rewrite <- Wf_Add_iff in Hvm; eauto.
     destruct Hvm as [Hvx0 [Hve Hvm]].
     unfold Add in *; rewrite H0 in *.
     apply add_in_iff in HIn as [Heq | HIn].
     -- rewrite Heq in *.
        exists e.
        rewrite H0; rewrite add_shadow.
-       apply valid_add_notin_spec; auto.
+       apply Wf_add_notin; auto.
        repeat split; auto.
-       eapply Key.valid_eq; eauto; try reflexivity.
+       eapply Key.Wf_iff; eauto; try reflexivity.
        now symmetry.
     -- apply (IHm1 HIn) in Hvm as [v Hvm].
        destruct (Key.eq_dec x x0) as [Heq | Hneq].
@@ -213,33 +208,30 @@ Proof.
        + exists v.
          rewrite H0.
          rewrite add_add_2; auto.
-         apply valid_add_notin_spec; auto.
+         apply Wf_add_notin; auto.
          rewrite add_in_iff; intros [Heq | HIn1]; contradiction.  
 Qed.
 
-Lemma valid_Add_spec (lb : Lvl.t) (x : Key.t) (v : Data.t) (m m' : t) :
+Lemma Wf_Add (lb: Lvl.t) (x: Key.t) (v: Data.t) (m m': t) :
   Add x v m m' -> 
-  Key.valid lb x /\ Data.valid lb v /\ valid lb m -> valid lb m'.
+  Key.Wf lb x /\ Data.Wf lb v /\ Wf lb m -> Wf lb m'.
 Proof.
   unfold Add; intros Heq Hv.
   rewrite Heq.
-  now apply valid_add_spec.
+  now apply Wf_add.
 Qed.
 
+(** *** extra [shift] properties *)
 
-(** *** extra [shift] property *)
-
-
-Lemma shift_Empty_spec (lb k : Lvl.t) (m : t) :
-  Empty m -> eq (shift lb k m) m.
+Lemma shift_Empty (lb k: Lvl.t) (m: t) : Empty m -> eq (shift lb k m) m.
 Proof.
   intro HEmp; unfold shift.
   rewrite fold_Empty with (eqA := eq); auto.
   symmetry. 
-  now apply Empty_eq_spec. 
+  now apply Empty_eq. 
 Qed.
 
-Lemma shift_Add_spec_1 (lb k : Lvl.t) (key : Key.t) (v : Data.t) (m m' : t) :
+Lemma shift_Add_1 (lb k: Lvl.t) (key: Key.t) (v: Data.t) (m m': t) :
   ~ M.In key m -> Add key v m m' -> 
   eq (shift lb k m') (M.add (Key.shift lb k key) (Data.shift lb k v) (shift lb k m)).
 Proof.
@@ -249,13 +241,12 @@ Proof.
   - now apply shift_proper.
 Qed.
 
-Lemma shift_Empty_iff (lb k : Lvl.t) (m : t) :
-  Empty m <-> Empty (shift lb k m).
+Lemma shift_Empty_iff (lb k: Lvl.t) (m: t) : Empty m <-> Empty (shift lb k m).
 Proof.
   split; intro HEmp.
-  - now rewrite shift_Empty_spec.
+  - now rewrite shift_Empty.
   - revert HEmp; induction m using map_induction; intro HEmp; auto.
-    rewrite shift_Add_spec_1 in HEmp; eauto.
+    rewrite shift_Add_1 in HEmp; eauto.
     exfalso; apply (HEmp (Key.shift lb k x) (Data.shift lb k e)).
     now apply add_1.
 Qed.
@@ -264,113 +255,111 @@ Qed.
 Proof.
   intros lb' lb Heqlb k' k Heqk m m' Heqm; subst.
   revert m' Heqm; induction m using map_induction; intros.
-  - repeat rewrite shift_Empty_spec; auto.
+  - repeat rewrite shift_Empty; auto.
     now rewrite <- Heqm.
-  - rewrite shift_Add_spec_1; eauto.
+  - rewrite shift_Add_1; eauto.
     symmetry.
-    rewrite shift_Add_spec_1; eauto; try reflexivity.
+    rewrite shift_Add_1; eauto; try reflexivity.
     unfold Add in *. 
     now rewrite <- Heqm.
 Qed.
 
-Lemma shift_add_notin_spec (lb k : Lvl.t) (x : Key.t) (v : Data.t) (m : t) :
+Lemma shift_add_notin (lb k: Lvl.t) (x: Key.t) (v: Data.t) (m: t) :
   ~ M.In x m ->  
-  eq (shift lb k (M.add x v m)) 
-      (M.add (Key.shift lb k x) (Data.shift lb k v) (shift lb k m)).
+  eq (shift lb k (M.add x v m)) (M.add (Key.shift lb k x) (Data.shift lb k v) (shift lb k m)).
 Proof.
   intro HIn; unfold shift.
   rewrite fold_add with (eqA := eq) (i := M.empty); eauto; try reflexivity.
   now apply shift_proper.
 Qed.
 
-Lemma shift_Add_spec_2 (lb k : Lvl.t) (key : Key.t) (v : Data.t) (m m' : t) :
+Lemma shift_Add_2 (lb k: Lvl.t) (key: Key.t) (v: Data.t) (m m': t) :
   ~ M.In key m -> Add key v m m' ->
   Add (Key.shift lb k key) (Data.shift lb k v) (shift lb k m) (shift lb k m').
 Proof.
   unfold Add; intros HnIn HAdd. 
-  now rewrite shift_Add_spec_1; eauto.
+  now rewrite shift_Add_1; eauto.
 Qed.
 
-Lemma shift_add_spec (lb k : Lvl.t) (x : Key.t) (v : Data.t) (m : t) :
-  eq (shift lb k (M.add x v m)) 
-      (M.add (Key.shift lb k x) (Data.shift lb k v) (shift lb k m)).
+Lemma shift_add (lb k: Lvl.t) (x: Key.t) (v: Data.t) (m: t) :
+  eq (shift lb k (M.add x v m)) (M.add (Key.shift lb k x) (Data.shift lb k v) (shift lb k m)).
 Proof.
   destruct (In_dec m x) as [HIn | HnIn].
   - revert HIn; induction m using map_induction; intro.
     -- exfalso.
-       rewrite Empty_eq_spec in *; auto.
+       rewrite Empty_eq in *; auto.
        now apply not_in_empty in HIn.
     -- unfold Add in H0; rewrite H0 in *; clear H0.
        apply add_in_iff in HIn as [Heq | HIn].
        + rewrite Heq in *.
          rewrite add_shadow.
-         repeat rewrite shift_add_notin_spec; auto.
+         repeat rewrite shift_add_notin; auto.
          now rewrite add_shadow.
        + destruct (Key.eq_dec x x0) as [Heq | Hneq].
          ++ rewrite Heq in HIn. 
             contradiction.
          ++ rewrite add_add_2; auto.
-            rewrite shift_add_notin_spec.
+            rewrite shift_add_notin.
             * rewrite IHm1; auto.
-              rewrite shift_add_notin_spec; auto.
+              rewrite shift_add_notin; auto.
               rewrite add_add_2; try reflexivity.
               rewrite <- Key.shift_eq_iff.
               intro Heq; symmetry in Heq.
               contradiction.
             * rewrite add_in_iff.
               intros [Heq | HIn0]; contradiction.
-  - now apply shift_add_notin_spec.
+  - now apply shift_add_notin.
 Qed.
 
-Lemma shift_Add_spec (lb k : Lvl.t) (key : Key.t) (v : Data.t) (m m' : t) :
+Lemma shift_Add (lb k: Lvl.t) (key: Key.t) (v: Data.t) (m m': t) :
   Add key v m m' -> 
   eq (shift lb k m') (M.add (Key.shift lb k key) (Data.shift lb k v) (shift lb k m)).
 Proof.
   unfold Add; intro Heq.
   rewrite Heq.
-  now apply shift_add_spec. 
+  now apply shift_add. 
 Qed.
   
-Lemma shift_in_spec_1 (lb k : Lvl.t) (key : Key.t) (m : t) :
+Lemma shift_in_1 (lb k: Lvl.t) (key: Key.t) (m: t) :
   M.In key m -> M.In (Key.shift lb k key) (shift lb k m).
 Proof.
   induction m using map_induction; intro HIn.
-  - rewrite Empty_eq_spec in HIn; auto.
+  - rewrite Empty_eq in HIn; auto.
     apply not_in_empty in HIn.
     now exfalso.
   - unfold Add in *; rewrite H0 in *; clear H0.
-    rewrite shift_add_spec.
+    rewrite shift_add.
     rewrite add_in_iff in *.
     destruct HIn as [Heq | HIn]; auto.
     left.
     now rewrite <- Key.shift_eq_iff.
 Qed.
 
-Lemma shift_in_spec_2 (lb k : Lvl.t) (key : Key.t) (m : t) :
+Lemma shift_in_2 (lb k: Lvl.t) (key: Key.t) (m: t) :
   M.In (Key.shift lb k key) (shift lb k m) -> M.In key m.
 Proof.
   induction m using map_induction; intro HIn.
-  - rewrite shift_Empty_spec in HIn; auto.
-    rewrite Empty_eq_spec in HIn; auto.
+  - rewrite shift_Empty in HIn; auto.
+    rewrite Empty_eq in HIn; auto.
     apply not_in_empty in HIn.
     now exfalso.
   - unfold Add in *; rewrite H0 in *; clear H0.
-    rewrite shift_add_notin_spec in *; auto.
+    rewrite shift_add_notin in *; auto.
     rewrite add_in_iff in *.
     destruct HIn as [Heq | HIn]; auto.
     left.
     now rewrite <- Key.shift_eq_iff in Heq.
 Qed.
 
-Lemma shift_in_iff (lb k : Lvl.t) (key : Key.t) (m : t) : 
+Lemma shift_in_iff (lb k: Lvl.t) (key: Key.t) (m: t) : 
   M.In key m <-> M.In (Key.shift lb k key) (shift lb k m).
 Proof. 
   split; intro HIn.
-  - apply (shift_in_spec_1 _ _ _ _ HIn).
-  - apply (shift_in_spec_2 lb k _ _ HIn).
+  - apply (shift_in_1 _ _ _ _ HIn).
+  - apply (shift_in_2 lb k _ _ HIn).
 Qed.
 
-Lemma shift_notin_iff (lb k : Lvl.t) (key : Key.t) (m : t) : 
+Lemma shift_notin_iff (lb k: Lvl.t) (key: Key.t) (m: t) : 
   ~ M.In key m <-> ~ M.In (Key.shift lb k key) (shift lb k m).
 Proof.
   split; intros HnIn HIn; apply HnIn.
@@ -378,16 +367,16 @@ Proof.
   - now rewrite <- shift_in_iff.
 Qed.
 
-Lemma shift_find_spec_1 (lb k : Lvl.t) (key : Key.t) (v : Data.t) (m : t) : 
+Lemma shift_find_1 (lb k: Lvl.t) (key: Key.t) (v: Data.t) (m: t) : 
   M.find key m = Some v -> 
   M.find (Key.shift lb k key) (shift lb k m) = Some (Data.shift lb k v).
 Proof.
   induction m using map_induction; intro Hfm.
-  - rewrite Empty_eq_spec in Hfm; auto. 
+  - rewrite Empty_eq in Hfm; auto. 
     rewrite empty_o in *.
     inversion Hfm.
   - unfold Add in H0; rewrite H0 in *; clear H0.
-    rewrite shift_add_spec.
+    rewrite shift_add.
     destruct (Key.eq_dec x key) as [Heq | Hneq].
     -- rewrite add_eq_o in *; auto.
        + now inversion Hfm.
@@ -396,17 +385,16 @@ Proof.
        now rewrite <- Key.shift_eq_iff.
 Qed.
 
-Lemma shift_find_spec_2 (lb k : Lvl.t) (key : Key.t) (v : Data.t) (m : t) : 
-  M.find (Key.shift lb k key) (shift lb k m) = Some (Data.shift lb k v) -> 
-  M.find key m = Some v.
+Lemma shift_find_2 (lb k: Lvl.t) (key: Key.t) (v: Data.t) (m: t) : 
+  M.find (Key.shift lb k key) (shift lb k m) = Some (Data.shift lb k v) -> M.find key m = Some v.
 Proof.
   induction m using map_induction; intro Hfm.
-  - rewrite shift_Empty_spec in Hfm; auto.
-    rewrite Empty_eq_spec in Hfm; auto.
+  - rewrite shift_Empty in Hfm; auto.
+    rewrite Empty_eq in Hfm; auto.
     rewrite empty_o in Hfm.
     inversion Hfm.
   - unfold Add in *; rewrite H0 in *; clear H0.
-    rewrite shift_add_spec in Hfm.
+    rewrite shift_add in Hfm.
     destruct (Key.eq_dec x key) as [Heq | Hneq].
     -- rewrite add_eq_o in *; auto.
        + inversion Hfm; f_equal. 
@@ -418,26 +406,24 @@ Proof.
        now rewrite <- Key.shift_eq_iff.
 Qed.
 
-Lemma shift_find_iff (lb k : Lvl.t) (key : Key.t) (v : Data.t) (m : t) : 
-  M.find key m = Some v <-> 
-  M.find (Key.shift lb k key) (shift lb k m) = Some (Data.shift lb k v).
+Lemma shift_find_iff (lb k: Lvl.t) (key: Key.t) (v: Data.t) (m: t) : 
+  M.find key m = Some v <-> M.find (Key.shift lb k key) (shift lb k m) = Some (Data.shift lb k v).
 Proof.
   split; intro Hfm.
-  - apply (shift_find_spec_1 _ _ _ _ _ Hfm).
-  - apply (shift_find_spec_2 lb k _ _ _ Hfm).
+  - apply (shift_find_1 _ _ _ _ _ Hfm).
+  - apply (shift_find_2 lb k _ _ _ Hfm).
 Qed.
 
-Lemma shift_find_e_spec (lb k : Lvl.t) (x : Key.t) (v : Data.t) (m : t) :
-  M.find (Key.shift lb k x) (shift lb k m) = Some v -> 
-  exists v', Data.eq v (Data.shift lb k v').
+Lemma shift_find_e (lb k: Lvl.t) (x: Key.t) (v: Data.t) (m: t) :
+  M.find (Key.shift lb k x) (shift lb k m) = Some v -> exists v', Data.eq v (Data.shift lb k v').
 Proof.
   induction m using map_induction; intro Hfm.
-  - rewrite shift_Empty_spec in Hfm; auto.
-    rewrite Empty_eq_spec in Hfm; auto.
+  - rewrite shift_Empty in Hfm; auto.
+    rewrite Empty_eq in Hfm; auto.
     rewrite empty_o in Hfm.
     inversion Hfm.
   - unfold Add in *; rewrite H0 in *; clear H0.
-    rewrite shift_add_spec in Hfm.
+    rewrite shift_add in Hfm.
     destruct (Key.eq_dec (Key.shift lb k x0) (Key.shift lb k x)) as [Heq | Hneq].
     -- rewrite add_eq_o in Hfm; auto.
        inversion Hfm; subst.
@@ -446,8 +432,7 @@ Proof.
 Qed.   
 
 
-Lemma shift_eq_iff (lb k : Lvl.t) (m m1 : t) : 
-  eq m m1 <-> eq (shift lb k m) (shift lb k m1).
+Lemma shift_eq_iff (lb k: Lvl.t) (m m1 : t) : eq m m1 <-> eq (shift lb k m) (shift lb k m1).
 Proof.
   split; intro Heq.
   - now rewrite Heq.
@@ -467,74 +452,73 @@ Proof.
        now apply not_in_find.
 Qed.
 
-Lemma shift_in_e_spec (lb k : Lvl.t) (x : M.key) (m : t) : 
+Lemma shift_in_e (lb k: Lvl.t) (x : M.key) (m: t) : 
   M.In x (shift lb k m) -> exists (x' : M.key), x = Key.shift lb k x'.
 Proof.
   revert x; induction m using map_induction; intros y HIn.
-  - rewrite shift_Empty_spec in HIn; auto.
+  - rewrite shift_Empty in HIn; auto.
     exfalso; destruct HIn as [v HM]; now apply (H y v).
   - unfold Add in H0; rewrite H0 in *; clear H0.
-    rewrite shift_add_spec in HIn.
+    rewrite shift_add in HIn.
     apply add_in_iff in HIn as [Heq | Hneq]; auto.
     exists x. 
     apply Key.eq_leibniz in Heq.  
     now rewrite Heq.
 Qed.
 
-Lemma shift_find_e_spec_1 (m n : Lvl.t) (x : M.key) (d : Data.t) (o : t) :
+Lemma shift_find_e_1 (m n : Lvl.t) (x : M.key) (d : Data.t) (o : t) :
   M.find x (shift m n o) = Some d -> 
   (exists x', Key.eq x (Key.shift m n x')) /\ (exists d', (Data.eq d (Data.shift m n d'))).
 Proof.
   intro Hfi.
   assert (HIn : M.In x (shift m n o)). { now exists d; apply find_2. }
-  apply shift_in_e_spec in HIn; split; auto;
+  apply shift_in_e in HIn; split; auto;
   destruct HIn as [x' Heq]; subst.
   - now exists x'.
-  - now apply shift_find_e_spec in Hfi.
+  - now apply shift_find_e in Hfi.
 Qed.
 
-Lemma valid_update_spec (lb : Lvl.t) (x : Key.t) (v : Data.t) (m : t) :
-  M.In x m -> valid lb m -> Data.valid lb v -> valid lb (M.add x v m).
+Lemma Wf_update (lb: Lvl.t) (x: Key.t) (v: Data.t) (m: t) :
+  M.In x m -> Wf lb m -> Data.Wf lb v -> Wf lb (M.add x v m).
 Proof.
   revert x v; induction m using map_induction; intros y v HIn Hvo Hvd.
-  - apply Empty_eq_spec in H; rewrite H in *.
+  - apply Empty_eq in H; rewrite H in *.
     inversion HIn.
     apply empty_mapsto_iff in H0; contradiction.
   - unfold Add in H0; rewrite H0 in *; clear H0.
-    apply valid_add_notin_spec in Hvo as [Hvx [Hve Hvm1]]; auto.
+    apply Wf_add_notin in Hvo as [Hvx [Hve Hvm1]]; auto.
     apply add_in_iff in HIn as [Heq | HIn]; subst.
     -- rewrite Heq in *. 
        rewrite add_shadow.
-       rewrite valid_add_notin_spec; auto.
+       rewrite Wf_add_notin; auto.
        repeat split; auto.
-       now eapply Key.valid_eq; eauto.
+       now eapply Key.Wf_iff; eauto.
     -- destruct (Key.eq_dec y x) as [Heq| Hneq].
        + rewrite Heq in *. contradiction.
        + rewrite add_add_2; auto.
          eapply IHm1 in Hvm1; eauto.
-         rewrite valid_add_notin_spec; auto.
+         rewrite Wf_add_notin; auto.
          rewrite add_in_iff; intros [Hc | Hc]; subst; contradiction.
 Qed.
 
-Lemma shift_Add_iff (lb k : Lvl.t) (key : Key.t) (v : Data.t) (m m' : t) :
-  Add key v m m' <->
-  Add (Key.shift lb k key) (Data.shift lb k v) (shift lb k m) (shift lb k m').
+Lemma shift_Add_iff (lb k: Lvl.t) (key: Key.t) (v: Data.t) (m m': t) :
+  Add key v m m' <-> Add (Key.shift lb k key) (Data.shift lb k v) (shift lb k m) (shift lb k m').
 Proof.
   unfold Add; split; intro HAdd.
   - rewrite HAdd.
-    now rewrite shift_add_spec.
-  - rewrite <- shift_add_spec in HAdd.
+    now rewrite shift_add.
+  - rewrite <- shift_add in HAdd.
     now rewrite <- shift_eq_iff in HAdd.
 Qed.
 
-Lemma shift_remove_spec (lb k : Lvl.t) (x : Key.t) (t : t) :
+Lemma shift_remove (lb k: Lvl.t) (x: Key.t) (t : t) :
   eq (M.remove (Key.shift lb k x) (shift lb k t)) (shift lb k (M.remove x t)).
 Proof.
   induction t using map_induction.
   - assert (HnIn : ~ M.In (Key.shift lb k x) (shift lb k t0)).
     { 
       apply shift_notin_iff.
-      rewrite Empty_eq_spec; auto.
+      rewrite Empty_eq; auto.
       now apply not_in_empty.
     }
     apply shift_notin_iff in HnIn as HnIn'.
@@ -544,23 +528,23 @@ Proof.
     destruct (Key.eq_dec x0 x) as [Heq | Hneq].
     -- symmetry.
        rewrite Heq at 1.
-       rewrite shift_add_spec.
+       rewrite shift_add.
        rewrite (Key.shift_eq_iff lb k) in Heq.
        rewrite Heq.
        now repeat rewrite remove_add_1.
     -- rewrite remove_add_2; auto.
-       repeat rewrite shift_add_spec; auto.
+       repeat rewrite shift_add; auto.
        rewrite remove_add_2.
        + now rewrite IHt1.
        + now rewrite <- Key.shift_eq_iff.
 Qed.
 
-Lemma shift_zero_refl (lb : Lvl.t) (t : t) : eq (shift lb 0 t) t.
+Lemma shift_zero_refl (lb: Lvl.t) (t : t) : eq (shift lb 0 t) t.
 Proof.
   induction t using map_induction.
-  - now apply shift_Empty_spec.
+  - now apply shift_Empty.
   - unfold Add in *; rewrite H0; clear H0.
-    rewrite shift_add_spec.
+    rewrite shift_add.
     rewrite IHt1.
     rewrite Key.shift_zero_refl.
     assert (Hzr : Data.shift lb 0 e = e). 
@@ -573,9 +557,9 @@ Lemma shift_trans (lb k k' : Lvl.t) (t : t) :
   eq (shift lb k (shift lb k' t)) (shift lb (k + k') t).
 Proof.
   induction t using map_induction. 
-  - now repeat rewrite shift_Empty_spec; auto.
+  - now repeat rewrite shift_Empty; auto.
   - unfold Add in *; rewrite H0; clear H0.
-    repeat rewrite shift_add_spec; auto.
+    repeat rewrite shift_add; auto.
     rewrite Key.shift_trans.
     rewrite IHt1.
 
@@ -589,9 +573,9 @@ Lemma shift_permute (lb k k' : Lvl.t) (t : t) :
   eq (shift lb k (shift lb k' t)) (shift lb k' (shift lb k t)).
 Proof.
   induction t using map_induction.
-  - now repeat rewrite shift_Empty_spec; auto.
+  - now repeat rewrite shift_Empty; auto.
   - unfold Add in *; rewrite H0; clear H0.
-    repeat rewrite shift_add_spec; auto.
+    repeat rewrite shift_add; auto.
     rewrite Key.shift_permute.
     rewrite IHt1.
 
@@ -606,9 +590,9 @@ Lemma shift_unfold (lb k k' : Lvl.t) (t : t) :
   eq (shift lb (k + k') t) (shift (lb + k) k' (shift lb k t)). 
 Proof.
   induction t using map_induction. 
-  - now repeat rewrite shift_Empty_spec; auto.
+  - now repeat rewrite shift_Empty; auto.
   - unfold Add in *; rewrite H0; clear H0.
-    repeat rewrite shift_add_spec; auto.
+    repeat rewrite shift_add; auto.
     rewrite Key.shift_unfold.
     rewrite IHt1.
 
@@ -623,9 +607,9 @@ Lemma shift_unfold_1 (k k' k'' : Lvl.t) (t : t) :
   eq (shift k' (k'' - k') (shift k  (k' - k) t)) (shift k (k'' - k) t).
 Proof.
   intros Hle Hle1; induction t using map_induction. 
-  - now repeat rewrite shift_Empty_spec; auto.
+  - now repeat rewrite shift_Empty; auto.
   - unfold Add in *; rewrite H0; clear H0.
-    repeat rewrite shift_add_spec; auto.
+    repeat rewrite shift_add; auto.
     rewrite Key.shift_unfold_1; auto.
     rewrite IHt1.
 
@@ -636,66 +620,66 @@ Proof.
 Qed.
 
 
-(** **** Interaction property between [valid] and [shift]  *)
+(** **** Interaction property between [Wf] and [shift]  *)
 
-Lemma valid_weakening (k k' : Lvl.t) (t : t) : (k <= k') -> valid k t -> valid k' t.
+Lemma Wf_weakening (k k' : Lvl.t) (t : t) : (k <= k') -> Wf k t -> Wf k' t.
 Proof.
   induction t using map_induction; intros Hle Hvt.
-  - now apply valid_Empty_spec.
+  - now apply Wf_Empty.
   - unfold Add in *; rewrite H0 in *; clear H0.
-    rewrite valid_add_notin_spec in *; auto.
+    rewrite Wf_add_notin in *; auto.
     destruct Hvt as [Hv [Hv' Hvt1]]. 
     repeat split; auto.
-    -- now apply Key.valid_weakening with k. 
-    -- now apply Data.valid_weakening with k.
+    -- now apply Key.Wf_weakening with k. 
+    -- now apply Data.Wf_weakening with k.
 Qed.
 
-Lemma shift_preserves_valid_1 (lb k k' : Lvl.t) (t : t) : 
-  valid k t -> valid (k + k') (shift lb k' t).
+Lemma shift_preserves_wf_1 (lb k k' : Lvl.t) (t : t) : 
+  Wf k t -> Wf (k + k') (shift lb k' t).
 Proof.
   induction t using map_induction; intro Hvt.
-  - rewrite shift_Empty_spec; auto.
-    now rewrite valid_Empty_iff.
-  - eapply valid_Add_iff in Hvt as [Hv [Hv' Hvt']]; eauto.
-    rewrite shift_Add_spec; eauto.
-    rewrite valid_add_notin_spec; auto.
+  - rewrite shift_Empty; auto.
+    now rewrite Wf_Empty_iff.
+  - eapply Wf_Add_iff in Hvt as [Hv [Hv' Hvt']]; eauto.
+    rewrite shift_Add; eauto.
+    rewrite Wf_add_notin; auto.
     -- repeat split; auto.
-       + now apply Key.shift_preserves_valid_1.
-       + now apply Data.shift_preserves_valid_1.
+       + now apply Key.shift_preserves_wf_1.
+       + now apply Data.shift_preserves_wf_1.
     -- now apply shift_notin_iff.
 Qed.
 
-Lemma shift_preserves_valid_gen (lb lb' k k' : Lvl.t) (t : t) :
+Lemma shift_preserves_wf_gen (lb lb' k k' : Lvl.t) (t : t) :
   k <= k' -> lb <= lb' -> k <= lb -> k' <= lb' -> k' - k = lb' - lb -> 
-  valid lb t -> valid lb' (shift k (k' - k) t).
+  Wf lb t -> Wf lb' (shift k (k' - k) t).
 Proof.
   intros Hle Hle1 Hle2 Hle3 Heq; induction t using map_induction; intro Hvt.
-  - rewrite shift_Empty_spec; auto.
-    now apply valid_Empty_spec.
-  - eapply valid_Add_iff in Hvt as [Hvx [Hve Hvt]]; eauto.
-    rewrite shift_Add_spec; eauto.
-    rewrite valid_add_notin_spec.
+  - rewrite shift_Empty; auto.
+    now apply Wf_Empty.
+  - eapply Wf_Add_iff in Hvt as [Hvx [Hve Hvt]]; eauto.
+    rewrite shift_Add; eauto.
+    rewrite Wf_add_notin.
     -- repeat split; auto.
-        + now apply Key.shift_preserves_valid_gen with (lb := lb).
-        + now apply Data.shift_preserves_valid_gen with (lb := lb).
+        + now apply Key.shift_preserves_wf_gen with (m := lb).
+        + now apply Data.shift_preserves_wf_gen with (m := lb).
     -- now apply shift_notin_iff.
 Qed.
 
-Lemma shift_preserves_valid_2 (lb lb' : Lvl.t) (t : t) :
-  lb <= lb' -> valid lb t -> valid lb' (shift lb (lb' - lb) t).
+Lemma shift_preserves_wf_2 (lb lb' : Lvl.t) (t : t) :
+  lb <= lb' -> Wf lb t -> Wf lb' (shift lb (lb' - lb) t).
 Proof. 
   intros Hle Hvt. 
-  apply (shift_preserves_valid_gen lb lb' lb lb'); auto.
+  apply (shift_preserves_wf_gen lb lb' lb lb'); auto.
 Qed.
 
-Lemma shift_preserves_valid (k k' : Lvl.t) (t : t) : valid k t -> valid (k + k') (shift k k' t).
-Proof. intro Hvt; now apply shift_preserves_valid_1. Qed.
+Lemma shift_preserves_wf (k k' : Lvl.t) (t : t) : Wf k t -> Wf (k + k') (shift k k' t).
+Proof. intro Hvt; now apply shift_preserves_wf_1. Qed.
 
-Lemma shift_preserves_valid_zero (k : Lvl.t) (t : t) : valid k t -> valid k (shift k 0 t).
+Lemma shift_preserves_wf_zero (k : Lvl.t) (t : t) : Wf k t -> Wf k (shift k 0 t).
 Proof. 
   intro Hvt. 
   replace k with (k + 0) by lia. 
-  now apply shift_preserves_valid_1. 
+  now apply shift_preserves_wf_1. 
 Qed.
 
 
@@ -703,56 +687,55 @@ End IsLvlMapKD.
 
 
 (** ** Bindless Leveled Map Implementation *)
-Module IsBdlLvlMapKD  
-  (Key : IsBdlLvlOTWL) (Data : IsBdlLvlETWL) 
-  (M : Interface.S Key) (MO : MapInterface Key Data M) <: IsBdlLvlMapKDInterface Key Data M MO.
+Module IsBdlLvlMapKD (Key : IsBdlLvlOTWL) (Data : IsBdlLvlETWL) (M : Interface.S Key) 
+                     (MO : MapInterface Key Data M) <: IsBdlLvlMapKDInterface Key Data M MO.
 
 Include IsLvlMapKD Key Data M MO.
 Import MO OP.P.  
 
-Lemma valid_in_iff (m n : Lvl.t) (x : M.key) (t : t) :
-  valid m t -> M.In x (shift m n t) <-> M.In x t.
+Lemma Wf_in_iff (m n : Lvl.t) (x : M.key) (t : t) :
+  Wf m t -> M.In x (shift m n t) <-> M.In x t.
 Proof.
   revert x; induction t using map_induction; intros y Hvo; split; intro HIn.
-  - rewrite shift_Empty_spec in HIn; auto.
-  - rewrite shift_Empty_spec; auto.
+  - rewrite shift_Empty in HIn; auto.
+  - rewrite shift_Empty; auto.
   - unfold Add in *; rewrite H0 in *; clear H0. 
-    apply valid_add_notin_spec in Hvo as [Hvk [Hvd Hv]]; auto.
-    rewrite shift_add_notin_spec in HIn; auto.
+    apply Wf_add_notin in Hvo as [Hvk [Hvd Hv]]; auto.
+    rewrite shift_add_notin in HIn; auto.
     rewrite add_in_iff in *; destruct HIn as [Heq | HIn]; subst.
     -- left; rewrite <- Heq. 
-       now rewrite Key.shift_valid_refl; auto.
+       now rewrite Key.shift_wf_refl; auto.
     -- right. rewrite <- IHt1; eauto.
   - unfold Add in *; rewrite H0 in *; clear H0. 
-    apply valid_add_notin_spec in Hvo as [Hvk [Hvd Hv]]; auto.
-    rewrite shift_add_notin_spec; auto.
+    apply Wf_add_notin in Hvo as [Hvk [Hvd Hv]]; auto.
+    rewrite shift_add_notin; auto.
     rewrite add_in_iff in *; destruct HIn as [Heq | HIn]; subst.
     -- left; rewrite <- Heq. 
-       now rewrite Key.shift_valid_refl; auto.
+       now rewrite Key.shift_wf_refl; auto.
     -- right. rewrite IHt1; eauto.
 Qed.
 
-Lemma shift_valid_refl (lb k : Lvl.t) (t : t) : valid lb t -> eq (shift lb k t) t.
+Lemma shift_wf_refl (lb k: Lvl.t) (t : t) : Wf lb t -> eq (shift lb k t) t.
 Proof.
   induction t using map_induction; intro Hvt.
-  - now apply shift_Empty_spec.
+  - now apply shift_Empty.
   - unfold Add in *; rewrite H0 in *; clear H0.
-    apply valid_add_notin_spec in Hvt as [Hvx [Hve Hvt]]; auto.
-    rewrite shift_add_spec.
+    apply Wf_add_notin in Hvt as [Hvx [Hve Hvt]]; auto.
+    rewrite shift_add.
     rewrite IHt1; auto.
-    rewrite Key.shift_valid_refl; auto. 
-    eapply Data.shift_valid_refl in Hve.
+    rewrite Key.shift_wf_refl; auto. 
+    eapply Data.shift_wf_refl in Hve.
     apply Data.eq_leibniz in Hve. 
     now rewrite Hve.
 Qed.
 
-Lemma shift_find_valid_spec (lb k : Lvl.t) (x : M.key) (m m' : t) :
-  Key.valid lb x -> M.In x m ->
+Lemma shift_find_Wf (lb k: Lvl.t) (x : M.key) (m m': t) :
+  Key.Wf lb x -> M.In x m ->
   M.find x m = M.find x m' -> M.find x (shift lb k m) = M.find x (shift lb k m').
 Proof.
   intros Hvk HIn Hfi. 
   destruct HIn as [v HfV]; apply find_1 in HfV.
-  rewrite <- (Key.shift_valid_refl lb k x); auto.
+  rewrite <- (Key.shift_wf_refl lb k x); auto.
   apply (shift_find_iff lb k) in HfV as HfV1.
   rewrite HfV1; symmetry.
   rewrite <- shift_find_iff.
@@ -767,18 +750,18 @@ End IsBdlLvlMapKD.
 
 Module MakeLvlMapKD (Key : IsLvlOTWL) (Data : IsLvlETWL) <: IsLvlET.
   
-  Module Raw := MMaps.OrdList.Make Key.
-  Module Ext := MapET Key Data Raw.
-  Include IsLvlMapKD Key Data Raw Ext.
-  Include OP.P.
+Module Raw := MMaps.OrdList.Make Key.
+Module Ext := MapET Key Data Raw.
+Include IsLvlMapKD Key Data Raw Ext.
+Include OP.P.
 
 End MakeLvlMapKD.
 
 Module MakeBdlLvlMapKD  (Key : IsBdlLvlOTWL) (Data : IsBdlLvlETWL) <: IsBdlLvlET.
   
-  Module Raw := MMaps.OrdList.Make Key.
-  Module Ext := MapET Key Data Raw.
-  Include IsBdlLvlMapKD Key Data Raw Ext.
-  Include OP.P.
+Module Raw := MMaps.OrdList.Make Key.
+Module Ext := MapET Key Data Raw.
+Include IsBdlLvlMapKD Key Data Raw Ext.
+Include OP.P.
 
 End MakeBdlLvlMapKD.
