theories/Set/Setkit/SetOTwL.v
@@ -1,319 +1,285 @@
 From Coq Require Import MSets Classical_Prop.
 From DeBrLevel Require Import SetOTwLInterface.
 
+(** * Implementation - [MSet] extension *)
+
+(** ** Extension of [MSet] *)
 Module SetOTWithLeibniz (Elt : MSetList.OrderedTypeWithLeibniz) <: (SetOTWithLeibnizInterface Elt).
 
+Include MSetList.MakeWithLeibniz Elt.
+Include MSetProperties.WPropertiesOn Elt.
 
-  Include MSetList.MakeWithLeibniz Elt.
-  Include MSetProperties.WPropertiesOn Elt.
+(** *** Definitions *)
 
-  Section definition.
+Definition ltb (s s' : t) : bool :=
+  match compare s s' with
+    | Lt => true
+    | _  => false
+  end
+.
 
+Definition map (f : elt -> elt) (s : t) : t := fold (fun r acc => add (f r) acc) s empty.
 
-    Definition ltb (s s' : t) : bool :=
-      match compare s s' with
-        | Lt => true
-        | _  => false
-      end
-    .
+(** *** Properties *)
 
-    Definition map (f : elt -> elt) (s : t) : t :=
-      fold (fun r acc => add (f r) acc) s empty
-    .
+(** **** Some facts *)
 
+Fact Add_inv (x: elt) (s s': t) : Add x s s' -> add x s = s'.
+Proof. 
+  intros; apply Add_Equal in H; apply eq_leibniz in H; now subst.
+Qed.
 
-  End definition.
+#[export] Instance proper_1 (f: elt -> elt) :
+  Proper (Elt.eq ==> eq ==> eq) (fun (r0 : elt) (acc : t) => add (f r0) acc).
+Proof. 
+  repeat red; intros; rewrite H0; apply Elt.eq_leibniz in H.
+  now rewrite H. 
+Qed.
 
-  Section fact.
+Fact transpose_1 (f: elt -> elt) :
+  transpose eq (fun (r0 : elt) (acc : t) => add (f r0) acc).
+Proof.
+  repeat red; intros; split; repeat rewrite add_spec; intros [|[|]]; auto.
+Qed.
 
+Section props.
 
-    Lemma Add_inv : forall x s s', Add x s s' -> add x s = s'.
-    Proof. 
-      intros; apply Add_Equal in H; apply eq_leibniz in H; now subst.
-    Qed.
+Variable x y: elt.
+Variable s s': t.
 
-    #[global] 
-    Instance proper_1 : forall f,
-      Proper (Elt.eq ==> eq ==> eq) (fun (r0 : elt) (acc : t) => add (f r0) acc).
-    Proof. 
-      repeat red; intros; rewrite H0; apply Elt.eq_leibniz in H.
-       now rewrite H. Qed.
+(** **** [eq] and [lt] properties *)
 
-    Lemma transpose_1 : forall f,
-      transpose eq (fun (r0 : elt) (acc : t) => add (f r0) acc).
-    Proof.
-      repeat red; intros; split; repeat rewrite add_spec; intros [|[|]]; auto.
-    Qed.
+Lemma eqb_refl : equal s s = true.
+Proof. intros; rewrite equal_spec; reflexivity. Qed.
 
+Lemma add_eq_leibniz :
+  ~ In x s -> ~ In x s' -> s = s' <-> (add x s) = (add x s').
+Proof.
+  split.
+  - intros; subst; auto.
+  - intros. assert (eq (add x s) (add x s')) by now rewrite H1.
+    apply eq_leibniz; split; intros.
+    -- destruct (H2 a). destruct (Elt.eq_dec a x); subst.
+        + apply Elt.eq_leibniz in e; subst; contradiction.
+        + assert (In a (add x s') -> In a s').
+          { intros. apply add_spec in H6. destruct H6; subst; try contradiction; auto. }
+          apply H6. apply H4. apply add_spec; now right.
+    -- destruct (H2 a). destruct (Elt.eq_dec a x); subst.
+        + apply Elt.eq_leibniz in e; subst; contradiction.
+        + assert (In a (add x s) -> In a s).
+          { intros. apply add_spec in H6. destruct H6; subst; try contradiction; auto. }
+          apply H6. apply H5. apply add_spec; now right.
+Qed.
 
-  End fact.
+Lemma ltb_lt : ltb s s' = true <-> lt s s'.
+Proof.
+  split; intros.
+  - unfold ltb in *; destruct (compare s s') eqn:Heq; try now inversion H.
+    clear H. assert (CompSpec eq lt s s' (compare s s')) by apply compare_spec.
+    rewrite Heq in H; now inversion H.
+  - assert (StrictOrder lt) by apply lt_strorder;
+    assert (CompSpec eq lt s s' (compare s s')) by apply compare_spec; unfold ltb; 
+    destruct (compare s s') eqn:Heq; auto.
+    -- unfold CompSpec in H1; inversion H1; apply eq_leibniz in H2; subst.
+        inversion H0. repeat red in StrictOrder_Irreflexive; exfalso; apply (StrictOrder_Irreflexive s' H).
+    -- exfalso. inversion H0. repeat red in StrictOrder_Irreflexive,StrictOrder_Transitive.
+      inversion H1. apply (StrictOrder_Transitive s s' s) in H2; auto.
+      apply StrictOrder_Irreflexive in H2; inversion H2.
+Qed.
 
-  Section equality.
+Lemma gt_neq_nlt : ~ eq s s' -> ~ lt s s' -> lt s' s.
+Proof.
+  intros. assert (CompSpec eq lt s s' (compare s s')) by apply compare_spec.
+  destruct (compare s s'); inversion H1; auto; contradiction.
+Qed.
 
+(** **** [In] properties *)
 
-    Lemma eqb_refl : forall s, equal s s = true.
-    Proof. intros; rewrite equal_spec; reflexivity. Qed.
+Lemma diff_in_add_spec : In x s' -> (diff (add x s) s') = (diff s s').
+Proof.
+  intros; apply eq_leibniz; split; intros; rewrite diff_spec in *; destruct H0; split; auto.
+  - rewrite add_spec in H0; destruct H0; auto; rewrite H0 in *; contradiction.
+  - rewrite add_spec; auto.
+Qed.
 
-    Lemma add_eq_leibniz : forall s s' v,
-      ~ In v s -> ~ In v s' -> s = s' <-> (add v s) = (add v s').
-    Proof.
-      split.
-      - intros; subst; auto.
-      - intros. assert (eq (add v s) (add v s')) by now rewrite H1.
-        apply eq_leibniz; split; intros.
-        -- destruct (H2 a). destruct (Elt.eq_dec a v); subst.
-           + apply Elt.eq_leibniz in e; subst; contradiction.
-           + assert (In a (add v s') -> In a s').
-             { intros. apply add_spec in H6. destruct H6; subst; try contradiction; auto. }
-             apply H6. apply H4. apply add_spec; now right.
-        -- destruct (H2 a). destruct (Elt.eq_dec a v); subst.
-           + apply Elt.eq_leibniz in e; subst; contradiction.
-           + assert (In a (add v s) -> In a s).
-             { intros. apply add_spec in H6. destruct H6; subst; try contradiction; auto. }
-             apply H6. apply H5. apply add_spec; now right.
-    Qed.
+Lemma union_add_spec : (union (add x s) s') =  add x (union s s').
+Proof.
+  intros; apply eq_leibniz; split; rewrite union_spec; rewrite add_spec; intros.
+  - destruct H as [[|]|]; rewrite add_spec; auto;
+    rewrite union_spec; auto.
+  - rewrite union_spec in H; destruct H as [|[|]];
+    rewrite add_spec; auto.
+Qed.
 
+Lemma inter_in_add_spec : In x s' -> (inter (add x s) s') = add x (inter s s').
+Proof.
+  intros; apply eq_leibniz; split; rewrite inter_spec; rewrite add_spec; intros.
+  - destruct H0 as [[|] ].
+    -- rewrite add_spec; auto.
+    -- rewrite add_spec; rewrite inter_spec; auto.
+  - rewrite inter_spec in H0; destruct H0.
+    -- rewrite H0 in *; split; auto; rewrite add_spec; left; reflexivity.
+    -- destruct H0; split; auto; rewrite add_spec; auto.
+Qed.
 
-  End equality.
+Lemma diff_notin_add_spec : ~ In x s' -> (diff (add x s) s') = add x (diff s s').
+Proof.
+  intros; apply eq_leibniz; split; intros.
+  - rewrite diff_spec in *; destruct H0; rewrite add_spec in *;
+    destruct H0; auto. right; rewrite diff_spec; split; assumption.
+  - rewrite diff_spec; rewrite add_spec in *; destruct H0.
+    -- rewrite H0 in *; split; auto; apply Elt.eq_leibniz in H0; subst;
+        auto; now left.
+    --  rewrite diff_spec in H0; destruct H0; split; auto.
+Qed.
 
-  Section lt.
+Lemma inter_notin_add_spec : ~ In x s' -> (inter (add x s) s') =  (inter s s').
+Proof.
+  intros; apply eq_leibniz; split; rewrite inter_spec; intros.
+  - rewrite add_spec in H0; destruct H0; destruct H0.
+    -- rewrite H0 in *; contradiction.
+    -- rewrite inter_spec; split; assumption.
+  - rewrite inter_spec; destruct H0; split; auto.
+    rewrite add_spec; right; assumption.
+Qed.
 
+Lemma add_notin_spec : ~ In x (add y s) <-> x <> y /\ ~ In x s.
+Proof.
+  split; intros.
+  - split; unfold not in *; intros; 
+    apply H; apply add_spec; auto; subst;
+    now left.
+  - destruct H; unfold not in *; intros.
+    rewrite add_spec in H1; destruct H1; auto.
+    apply Elt.eq_leibniz in H1; subst; now apply H.
+Qed. 
 
-    Lemma ltb_lt : forall s s', ltb s s' = true <-> lt s s'.
-    Proof.
-      split; intros.
-      - unfold ltb in *; destruct (compare s s') eqn:Heq; try now inversion H.
-        clear H. assert (CompSpec eq lt s s' (compare s s')) by apply compare_spec.
-        rewrite Heq in H; now inversion H.
-      - assert (StrictOrder lt) by apply lt_strorder;
-        assert (CompSpec eq lt s s' (compare s s')) by apply compare_spec; unfold ltb; 
-        destruct (compare s s') eqn:Heq; auto.
-        -- unfold CompSpec in H1; inversion H1; apply eq_leibniz in H2; subst.
-           inversion H0. repeat red in StrictOrder_Irreflexive; exfalso; apply (StrictOrder_Irreflexive s' H).
-        -- exfalso. inversion H0. repeat red in StrictOrder_Irreflexive,StrictOrder_Transitive.
-          inversion H1. apply (StrictOrder_Transitive s s' s) in H2; auto.
-          apply StrictOrder_Irreflexive in H2; inversion H2.
-    Qed.
+Lemma union_notin_spec : ~ In x (union s s') <-> ~ In x s /\ ~ In x s'.
+Proof. 
+  split; unfold not; intros.
+  - split; intro; apply H; apply union_spec; auto.
+  - destruct H; apply union_spec in H0 as [H0 | H0]; auto. 
+Qed.
 
-    Lemma gt_neq_nlt : forall s s', ~ eq s s' -> ~ lt s s' -> lt s' s.
-    Proof.
-      intros. assert (CompSpec eq lt s s' (compare s s')) by apply compare_spec.
-      destruct (compare s s'); inversion H1; auto; contradiction.
-    Qed.
+Lemma diff_notin_spec : ~ In x (diff s s') <-> ~ In x s \/ In x s'.
+Proof.
+  unfold not; split; intros.
+  - apply NNPP; unfold not; intros. apply H. apply diff_spec; split.
+    -- apply NNPP; unfold not; intros. apply H0; left; auto.
+    -- unfold not; intros; apply H0. now right.
+  - apply diff_spec in H0 as [H0 H0']. destruct H; auto.
+Qed.
 
+Lemma singleton_notin_spec : ~ In x (singleton  y) <-> x <> y.
+Proof.
+  split; unfold not; intros.
+  - apply H; apply singleton_spec; subst; reflexivity.
+  - apply H; apply singleton_spec in H0; now apply Elt.eq_leibniz in H0.
+Qed.
+  
 
-  End lt.
+End props.
 
-  Section in_set.
+#[local] Hint Resolve eq_equiv transpose_1 proper_1 : core.
 
+(** **** [map] properties *)
 
-    Variable x : elt.
-    Variable s s' : t.
+Lemma map_Empty_spec (s: t) (f: elt -> elt) : Empty s -> map f s = empty.
+Proof.
+  intros; unfold map; apply empty_is_empty_1 in H. 
+  apply eq_leibniz in H; subst; now rewrite fold_empty.
+Qed.
 
-    Lemma diff_in_add_spec :
-      In x s' -> (diff (add x s) s') = (diff s s').
-    Proof.
-      intros; apply eq_leibniz; split; intros; rewrite diff_spec in *; destruct H0; split; auto.
-      - rewrite add_spec in H0; destruct H0; auto; rewrite H0 in *; contradiction.
-      - rewrite add_spec; auto.
-    Qed.
+Lemma map_empty_spec (f: elt -> elt) : map f empty = empty.
+Proof.
+  intros; unfold map; now rewrite fold_empty. 
+Qed.
 
-    Lemma union_add_spec :
-      (union (add x s) s') =  add x (union s s').
-    Proof.
-      intros; apply eq_leibniz; split; rewrite union_spec; rewrite add_spec; intros.
-      - destruct H as [[|]|]; rewrite add_spec; auto;
-        rewrite union_spec; auto.
-      - rewrite union_spec in H; destruct H as [|[|]];
-        rewrite add_spec; auto.
-    Qed.
+Lemma map_singleton_spec (x: elt) (f: elt -> elt) : map f (singleton x) = singleton (f x).
+Proof.
+  intros; unfold map. 
+  replace (singleton x) with (add x empty).
+  - apply eq_leibniz; rewrite fold_add; auto.
+    -- rewrite fold_empty; symmetry; apply singleton_equal_add.
+    -- unfold not; intros H; inversion H.
+  - apply eq_leibniz; apply singleton_equal_add.
+Qed.
 
-    Lemma inter_in_add_spec :
-      In x s' -> (inter (add x s) s') = add x (inter s s').
-    Proof.
-      intros; apply eq_leibniz; split; rewrite inter_spec; rewrite add_spec; intros.
-      - destruct H0 as [[|] ].
-        -- rewrite add_spec; auto.
-        -- rewrite add_spec; rewrite inter_spec; auto.
-      - rewrite inter_spec in H0; destruct H0.
-        -- rewrite H0 in *; split; auto; rewrite add_spec; left; reflexivity.
-        -- destruct H0; split; auto; rewrite add_spec; auto.
-    Qed.
+Lemma map_in_spec (x: elt) (s: t) (f: elt -> elt) : In x s -> In (f x) (map f s).
+Proof.
+  induction s using set_induction; intro HI.
+  - apply empty_is_empty_1 in H; apply eq_leibniz in H; subst.
+    inversion HI.
 
+  - intros; apply Add_inv in H0; subst; unfold map in *; rewrite add_spec in *.
+    rewrite fold_add; auto; rewrite add_spec. destruct HI; auto. 
+    apply Elt.eq_leibniz in H0; subst; now left.
+Qed.
 
-  End in_set.
+Lemma map_add_notin_spec (x: elt) (s: t) (f: elt -> elt) : 
+  ~ In x s -> map f (add x s) = add (f x) (map f s).
+Proof.
+  intros; apply eq_leibniz; unfold map; rewrite fold_add; now auto.
+Qed.
 
-  Section notin_set.
+Lemma map_add_in_spec (x: elt) (s: t) (f: elt -> elt) : In x s -> map f (add x s) = (map f s).
+Proof.
+  intros; apply eq_leibniz; unfold map; rewrite add_fold; now auto.
+Qed.
 
-    Variable x r r' : elt.
-    Variable s s' s1 s2 : t.
+Fact union_sym_leibniz (s s': t) : union s s' = union s' s.
+Proof.
+  apply eq_leibniz.
+  now rewrite union_sym.
+Qed.
 
-    Lemma diff_notin_add_spec :
-      ~ In x s' -> (diff (add x s) s') = add x (diff s s').
-    Proof.
-      intros; apply eq_leibniz; split; intros.
-      - rewrite diff_spec in *; destruct H0; rewrite add_spec in *;
-        destruct H0; auto. right; rewrite diff_spec; split; assumption.
-      - rewrite diff_spec; rewrite add_spec in *; destruct H0.
-        -- rewrite H0 in *; split; auto; apply Elt.eq_leibniz in H0; subst;
-           auto; now left.
-        --  rewrite diff_spec in H0; destruct H0; split; auto.
-    Qed.
+Fact add_shadow_leibniz (x: elt) (s: t) : add x (add x s) = add x s.
+Proof.
+  apply eq_leibniz.
+  rewrite add_equal.
+  - reflexivity.
+  - rewrite add_spec; now left.
+Qed. 
 
-    Lemma inter_notin_add_spec :
-      ~ In x s' -> (inter (add x s) s') =  (inter s s').
-    Proof.
-      intros; apply eq_leibniz; split; rewrite inter_spec; intros.
-      - rewrite add_spec in H0; destruct H0; destruct H0.
-        -- rewrite H0 in *; contradiction.
-        -- rewrite inter_spec; split; assumption.
-      - rewrite inter_spec; destruct H0; split; auto.
-        rewrite add_spec; right; assumption.
-    Qed.
-
-    Lemma add_notin_spec :
-      ~ In r (add r' s) <-> r <> r' /\ ~ In r s.
-    Proof.
-      split; intros.
-      - split; unfold not in *; intros; 
-        apply H; apply add_spec; auto; subst;
-        now left.
-      - destruct H; unfold not in *; intros.
-        rewrite add_spec in H1; destruct H1; auto.
-        apply Elt.eq_leibniz in H1; subst; now apply H.
-    Qed. 
-
-    Lemma union_notin_spec :
-      ~ In r (union s1 s2) <-> ~ In r s1 /\ ~ In r s2.
-    Proof. 
-      split; unfold not; intros.
-      - split; intro; apply H; apply union_spec; auto.
-      - destruct H; apply union_spec in H0 as [H0 | H0]; auto. 
-    Qed.
-
-    Lemma diff_notin_spec :
-      ~ In r (diff s1 s2) <-> ~ In r s1 \/ In r s2.
-    Proof.
-      unfold not; split; intros.
-      - apply NNPP; unfold not; intros. apply H. apply diff_spec; split.
-        -- apply NNPP; unfold not; intros. apply H0; left; auto.
-        -- unfold not; intros; apply H0. now right.
-      - apply diff_spec in H0 as [H0 H0']. destruct H; auto.
-    Qed.
-
-    Lemma singleton_notin_spec :
-      ~ In r (singleton  r') <-> r <> r'.
-    Proof.
-      split; unfold not; intros.
-      - apply H; apply singleton_spec; subst; reflexivity.
-      - apply H; apply singleton_spec in H0; now apply Elt.eq_leibniz in H0.
-    Qed.
-
-
-  End notin_set.
-
-  Section map.
-
-
-    #[local] Hint Resolve eq_equiv transpose_1 proper_1 : core.
-
-    Lemma map_Empty_spec : forall f s,
-      Empty s -> map f s = empty.
-    Proof.
-      intros; unfold map; apply empty_is_empty_1 in H. 
-      apply eq_leibniz in H; subst; now rewrite fold_empty.
-    Qed.
-
-    Lemma map_empty_spec : forall f,
-      map f empty = empty.
-    Proof.
-      intros; unfold map; now rewrite fold_empty. 
-    Qed.
-
-    Lemma map_singleton_spec : forall f re,
-      map f (singleton re) = singleton (f re).
-    Proof.
-      intros; unfold map. 
-      replace (singleton re) with (add re empty).
-      - apply eq_leibniz; rewrite fold_add; auto.
-        -- rewrite fold_empty; symmetry; apply singleton_equal_add.
-        -- unfold not; intros H; inversion H.
-      - apply eq_leibniz; apply singleton_equal_add.
-    Qed.
-
-    Lemma map_in_spec : forall s f re,
-      In re s -> In (f re) (map f s).
-    Proof.
-      intros s; induction s using set_induction; intros f re HI.
-      - apply empty_is_empty_1 in H; apply eq_leibniz in H; subst.
-        inversion HI.
-
-      - intros; apply Add_inv in H0; subst; unfold map in *; rewrite add_spec in *.
-        rewrite fold_add; auto; rewrite add_spec. destruct HI; auto. 
-        apply Elt.eq_leibniz in H0; subst; now left.
-    Qed.
-
-    Lemma map_add_notin_spec : forall f re s,
-      ~ In re s -> map f (add re s) = add (f re) (map f s).
-    Proof.
-      intros; apply eq_leibniz; unfold map; rewrite fold_add; now auto.
-    Qed.
-
-    Lemma map_add_in_spec : forall f re s,
-      In re s -> map f (add re s) = (map f s).
-    Proof.
-      intros; apply eq_leibniz; unfold map; rewrite add_fold; now auto.
-    Qed.
-
-    Lemma map_union_spec : forall s s' f,
-      (map f (union s s')) = union (map f s) (map f s').
-    Proof.
-      intros; apply eq_leibniz; generalize s' f; clear s' f.
-      induction s using set_induction; intros s' f.
-      - split; intros.
-        -- apply empty_is_empty_1 in H; apply eq_leibniz in H; subst.
-          replace (union empty s') with s' in H0; unfold map in *. rewrite fold_empty.
-          + apply union_spec; auto.
-          + apply eq_leibniz; rewrite empty_union_1; eauto; reflexivity.
-
-        -- unfold map in *. apply empty_is_empty_1 in H; apply eq_leibniz in H; subst.
-          apply union_spec in H0 as [|].
-          + rewrite fold_empty in H; inversion H.
-          + replace (union empty s') with s'; auto.
-              apply eq_leibniz; rewrite empty_union_1; eauto; reflexivity.
-
-      - split; intros.
-        -- apply Add_inv in H0; subst; rewrite union_add_spec in H1; destruct (In_dec x s').
-          + rewrite map_add_in_spec in H1.
-            ++ apply IHs1 in H1. rewrite union_spec in *; destruct H1; auto.
-                left; rewrite map_add_notin_spec; auto. rewrite add_spec; auto.
-            ++ apply union_spec; now right.
-            + rewrite map_add_notin_spec in H1.
-              ++ rewrite add_spec in H1; rewrite union_spec; destruct H1.
-                * rewrite H0 in *; left; rewrite map_add_notin_spec; auto.
-                  rewrite add_spec; left; reflexivity.
-                * apply IHs1 in H0; rewrite union_spec in H0; destruct H0; auto.
-                  left; rewrite map_add_notin_spec; auto; rewrite add_spec; auto.
-              ++ rewrite union_notin_spec; split; assumption.
-        -- apply Add_inv in H0; subst; rewrite union_add_spec; rewrite union_spec in *; 
-          destruct (In_dec x s').
-          + rewrite map_add_in_spec.
-            ++ destruct H1.
-                * rewrite map_add_notin_spec in H0; auto; rewrite add_spec in H0; destruct H0.
-                  ** rewrite H0 in *; rewrite IHs1; rewrite union_spec; right.
-                    now apply map_in_spec.
-                  ** rewrite IHs1; rewrite union_spec; now left.
-                * rewrite IHs1; rewrite union_spec; now right.
-            ++ apply union_spec; auto.
-          + rewrite map_add_notin_spec.
-            ++ destruct H1.
-                * rewrite map_add_notin_spec in H0; auto; rewrite add_spec in *.
-                  destruct H0; auto; right; apply IHs1; rewrite union_spec; auto.
-                * rewrite add_spec; right; apply IHs1; rewrite union_spec; auto.
-            ++ apply union_notin_spec; split; assumption.
-    Qed.
-
-
-  End map.
+Lemma map_union_spec (s s': t) (f: elt -> elt) : 
+  (map f (union s s')) = union (map f s) (map f s').
+Proof.
+  apply eq_leibniz.
+  revert s f s'; clear; intro s. 
+  induction s using set_induction; intros f s'.
+  -  assert (HUn: union s s' = s').
+    -- apply eq_leibniz. 
+       rewrite empty_union_1; auto; reflexivity.
+    -- rewrite HUn.
+       rewrite (map_Empty_spec s); auto.
+       rewrite empty_union_1; auto.
+       reflexivity.
+  - apply Add_inv in H0; subst.
+    rewrite (map_add_notin_spec _ s1); auto.
+    do 2 rewrite union_add_spec.
+    destruct (In_dec x s') as [HIn | HnIn].
+    -- rewrite union_sym_leibniz; symmetry;
+       rewrite union_sym_leibniz; symmetry. 
+       apply add_remove in HIn as Heq.
+       apply eq_leibniz in Heq; rewrite <- Heq; clear Heq.
+       rewrite union_add_spec.
+       rewrite add_shadow_leibniz.
+       rewrite map_add_notin_spec.
+       + rewrite union_sym_leibniz. 
+         rewrite IHs1.
+         rewrite union_sym_leibniz.
+         symmetry.
+         rewrite map_add_notin_spec.
+         ++ rewrite union_add_spec.
+            now rewrite add_shadow_leibniz.
+         ++ rewrite remove_spec; intros []. 
+            apply H1; reflexivity.
+       + rewrite union_notin_spec; split; auto.
+         rewrite remove_spec; intros [].
+         apply H1; reflexivity.
+    -- rewrite map_add_notin_spec.
+       + now rewrite IHs1.
+       + rewrite union_notin_spec; split; assumption.
+Qed.
 
 End SetOTWithLeibniz.
