theories/Map/MapLevelInterface.v
@@ -1,0 +1,395 @@
+From Coq Require Import Structures.Equalities.
+From DeBrLevel Require Import Level LevelInterface MapExtInterface. 
+
+(** * Interface - Leveled Map
+
+  Based on the overlay [MapExt] we defined interfaces for maps with [shift] and [Wf].
+  The [shift] function is applied on all leveled elements (keys and/or data), and a map is 
+  well-formed under [k] if all leveled elements in it are also well-formed under [k]. For each interface we specify via the notation [?K/?D] the configuration of the map where [K] stands for keys and [D] for data. ? can be [OT] for ordered type, [ET] for equality type and [Lvl] for leved type.
+*)
+
+(** ** Leveled Map Interface - [OTK/LvlD] *)
+Module Type IsLvlMapDInterface (Key : OrderedTypeWithLeibniz) (Data : IsLvlETWL) 
+                               (M : Interface.S Key) (MO : MapInterface Key Data M) <: IsLvl MO.
+
+Include IsLvl MO.
+Import MO OP.P.
+
+Section specs.
+
+Variable k n p : Lvl.t.
+Variable x : M.key.
+Variable v : Data.t.
+Variable m m' : t.
+
+(** *** extra [Wf] specifications *)
+
+Parameter Wf_Empty : Empty m -> Wf k m.
+
+Parameter Wf_empty : Wf k M.empty.
+
+Parameter Wf_Add_iff : ~ M.In x m -> Add x v m m' ->  (Data.Wf k v /\ Wf k m <-> Wf k m').
+
+Parameter Wf_Add : Add x v m m' ->  (Data.Wf k v /\ Wf k m -> Wf k m').
+
+Parameter Wf_add_in : M.In x m -> Wf k m -> exists v, Wf k (M.add x v m).
+
+Parameter Wf_add : Data.Wf k v /\ Wf k m -> Wf k (M.add x v m).
+
+Parameter Wf_find : Wf k m -> M.find x m = Some v -> Data.Wf k v.
+
+Parameter Wf_update : M.In x m -> Wf k m -> Data.Wf k v -> Wf k (M.add x v m).
+
+(** *** extra [shift] specifications *)
+
+Parameter shift_Empty_iff : Empty m <-> Empty (shift k n m).
+
+Parameter shift_Empty : Empty m -> eq (shift k n m) m.
+
+Parameter shift_add : eq (shift k n (M.add x v m)) (M.add x (Data.shift k n v) (shift k n m)).
+
+Parameter shift_Add : Add x v m m' -> eq (shift k n m') (M.add x (Data.shift k n v) (shift k n m)).
+
+Parameter shift_Add_iff : Add x v m m' <-> Add x (Data.shift k n v) (shift k n m) (shift k n m').
+
+Parameter shift_remove : eq (M.remove x (shift k n m)) (shift k n (M.remove x m)).
+
+Parameter shift_in_iff :  M.In x m <-> M.In x (shift k n m).
+
+Parameter shift_notin_iff : ~ M.In x m <-> ~ M.In x (shift k n m).
+
+Parameter shift_find_iff : M.find x m = Some v <-> M.find x (shift k n m) = Some (Data.shift k n v).
+
+End specs.
+
+End IsLvlMapDInterface.
+
+
+(** ** Bindless Leveled Map Interface - [OTK/LvlD] *)
+Module Type IsBdlLvlMapDInterface (Key : OrderedTypeWithLeibniz) (Data : IsBdlLvlETWL) 
+                                  (M : Interface.S Key) (MO : MapInterface Key Data M) 
+                                  <: IsBdlLvl MO
+:= IsLvlMapDInterface Key Data M MO <+ IsBindlessLeveledEx MO.
+
+(** ** Alternative Leveled Map Interface - [OTK/LvlD]
+  Map with boolean version of [Wf] named [is_wf] 
+*)
+Module Type IsLvlFullMapDInterface (Key : OrderedTypeWithLeibniz) (Data : IsLvlFullETWL) 
+                                   (M : Interface.S Key) (MO : MapInterface Key Data M)
+:= (IsLvlMapDInterface Key Data M MO) <+ IsWFFull MO.
+
+(** ** Alternative Bindless Leveled Map Interface  - [OTK/LvlD] 
+  Map with boolean version of [Wf] named [is_Wf] 
+*)
+Module Type IsBdlLvlFullMapDInterface (Key : OrderedTypeWithLeibniz) (Data : IsBdlLvlFullETWL) 
+                                      (M : Interface.S Key) (MO : MapInterface Key Data M) 
+:=  (IsBdlLvlMapDInterface Key Data M MO) <+ IsWFFull MO.
+
+
+(** ---- *)
+
+
+(** ** Leveled Map Interface - [LvlK/ETD] *)
+Module Type IsLvlMapKInterface (Key : IsLvlOTWL) (Data : EqualityType) 
+                               (M : Interface.S Key) (MO : MapInterface Key Data M) <: IsLvl MO.
+
+Include IsLvl MO.
+Import MO OP.P.
+
+Section specs.
+
+Variable k n p : Lvl.t.
+Variable x : M.key.
+Variable v : Data.t.
+Variable m m' : t.
+
+(** *** extra [Wf] specifications *)
+
+Parameter Wf_Empty : Empty m -> Wf k m.
+
+Parameter Wf_Empty_iff : Empty m -> Wf k m <-> True.
+
+Parameter Wf_empty : Wf k M.empty.
+
+Parameter Wf_add_iff : Key.Wf k x /\ Wf k m <-> Wf k (M.add x v m).
+
+Parameter Wf_add_in : M.In x m -> Wf k m -> exists v, Wf k (M.add x v m).
+
+Parameter Wf_Add_iff : Add x v m m' -> (Key.Wf k x /\ Wf k m <-> Wf k m').
+
+Parameter Wf_in : Wf k m -> M.In x m -> Key.Wf k x.
+
+(** *** extra [shift] specifications *)
+
+Parameter shift_Empty_iff : Empty m <-> Empty (shift k n m).
+
+Parameter shift_Empty : Empty m -> eq (shift k n m) m.
+
+Parameter shift_add : eq  (shift k n (M.add x v m)) (M.add (Key.shift k n x) v (shift k n m)).
+
+Parameter shift_Add : Add x v m m' -> eq (shift k n m') (M.add (Key.shift k n x) v (shift k n m)).
+
+Parameter shift_Add_iff : Add x v m m' <-> Add (Key.shift k n x) v (shift k n m) (shift k n m').
+
+Parameter shift_remove : eq (M.remove (Key.shift k n x) (shift k n m)) (shift k n (M.remove x m)).
+
+Parameter shift_in_e : M.In x (shift k n m) -> exists (x' : Key.t), x = Key.shift k n x'.
+
+Parameter shift_in_iff : M.In x m <-> M.In (Key.shift k n x) (shift k n m).
+
+Parameter shift_notin_iff : ~ M.In x m <-> ~ M.In (Key.shift k n x) (shift k n m).
+
+Parameter shift_find : M.find x m = M.find (Key.shift k n x) (shift k n m).
+
+End specs.
+
+End IsLvlMapKInterface.
+
+
+(** ** Bindless Leveled Map Interface - [LvlK/ETD] *)
+Module Type IsBdlLvlMapKInterface (Key : IsBdlLvlOTWL) (Data : EqualityType) 
+                                (M : Interface.S Key) (MO : MapInterface Key Data M) <: IsBdlLvl MO.
+
+Include IsLvlMapKInterface Key Data M MO.
+Import MO OP.P.
+
+Parameter Wf_in_iff : forall (m n : Lvl.t) (x : M.key) (t : t),
+  Wf m t -> M.In x (shift m n t) <-> M.In x t.
+
+Parameter shift_find_Wf : forall (k n : Lvl.t) (x : M.key) (m m' : t),
+  Key.Wf k x -> M.In x m ->
+  M.find x m = M.find x m' -> M.find x (shift k n m) = M.find x (shift k n m').
+
+Parameter shift_wf_refl : forall k n t, Wf k t -> eq (shift k n t) t.
+
+End IsBdlLvlMapKInterface.
+
+(** ** Alternative Leveled Map Interface - [LvlK/ETD] *)
+Module Type IsLvlFullMapKInterface (Key : IsLvlFullOTWL) (Data : EqualityType) 
+                                   (M : Interface.S Key) (MO : MapInterface Key Data M)
+:= (IsLvlMapKInterface Key Data M MO) <+ IsWFFull MO.
+
+(** ** Alternative Bindless Leveled Map Interface - [LvlK/ETD] *)
+Module Type IsBdlLvlFullMapKInterface (Key : IsBdlLvlFullOTWL) (Data : EqualityType)
+                                      (M : Interface.S Key) (MO : MapInterface Key Data M) 
+:=  (IsBdlLvlMapKInterface Key Data M MO) <+ IsWFFull MO.
+
+
+(** ---- *)
+
+(** ** Leveled Map Interface - [LvlK/LvlD] *)
+
+Module Type IsLvlMapKDInterface (Key : IsLvlOTWL) (Data : IsLvlETWL) 
+                                (M : Interface.S Key) (MO : MapInterface Key Data M) <: IsLvl MO.
+
+Include IsLvl MO.
+Import MO OP.P.
+
+Section specs.
+
+Variable k n p : Lvl.t.
+Variable x : M.key.
+Variable v : Data.t.
+Variable m m' : t.
+
+(** *** extra [Wf] specifications *)
+
+Parameter Wf_Empty : Empty m -> Wf k m.
+
+Parameter Wf_Empty_iff : Empty m -> Wf k m <-> True.
+
+Parameter Wf_empty : Wf k M.empty.
+
+Parameter Wf_add : Key.Wf k x /\ Data.Wf k v /\ Wf k m -> Wf k (M.add x v m).
+
+Parameter Wf_add_notin : ~ M.In x m -> 
+                         Wf k (M.add x v m) <-> Key.Wf k x /\ Data.Wf k v /\ Wf k m.
+
+Parameter Wf_add_in : M.In x m -> Wf k m -> exists v, Wf k (M.add x v m).
+
+Parameter Wf_Add_iff : ~ M.In x m -> 
+                       Add x v m m' -> (Key.Wf k x /\ Data.Wf k v /\ Wf k m <-> Wf k m').
+
+Parameter Wf_Add : Add x v m m' -> (Key.Wf k x /\ Data.Wf k v /\ Wf k m -> Wf k m').
+
+Parameter Wf_find : Wf k m -> M.find x m = Some v -> Key.Wf k x /\ Data.Wf k v.
+
+Parameter Wf_in : Wf k m -> M.In x m -> Key.Wf k x.
+
+Parameter Wf_update : M.In x m -> Wf k m -> Data.Wf k v -> Wf k (M.add x v m).
+
+(** *** extra [shift] specifications *)
+
+Parameter shift_Empty_iff : Empty m <-> Empty (shift k n m).
+
+Parameter shift_Empty : Empty m -> eq (shift k n m) m.
+
+Parameter shift_add :
+  eq (shift k n (M.add x v m)) (M.add (Key.shift k n x) (Data.shift k n v) (shift k n m)).
+
+Parameter shift_Add : Add x v m m' -> 
+  eq (shift k n m') (M.add (Key.shift k n x) (Data.shift k n v) (shift k n m)).
+
+Parameter shift_Add_iff : Add x v m m' <->
+  Add (Key.shift k n x) (Data.shift k n v) (shift k n m) (shift k n m').
+
+Parameter shift_remove : eq (M.remove (Key.shift k n x) (shift k n m)) (shift k n (M.remove x m)).
+
+Parameter shift_in_e : M.In x (shift k n m) -> exists (x' : Key.t), x = Key.shift k n x'.
+
+Parameter shift_in_iff :  M.In x m <-> M.In (Key.shift k n x) (shift k n m).
+
+Parameter shift_notin_iff : ~ M.In x m <-> ~ M.In (Key.shift k n x) (shift k n m).
+
+Parameter shift_find_iff :
+  M.find x m = Some v <->  M.find (Key.shift k n x) (shift k n m) = Some (Data.shift k n v).
+
+Parameter shift_find_e :
+  M.find (Key.shift k n x) (shift k n m) = Some v ->  exists v', Data.eq v (Data.shift k n v').
+
+Parameter shift_find_e_1 :
+  M.find x (shift k n m) = Some v ->  (exists x', Key.eq x (Key.shift k n x')) /\ 
+                                      (exists v', Data.eq v (Data.shift k n v')).
+
+End specs.
+
+End IsLvlMapKDInterface.
+
+(** ** Bindless Leveled Map Interface - [LvlK/LvlD] *)
+Module Type IsBdlLvlMapKDInterface (Key : IsBdlLvlOTWL) (Data : IsBdlLvlETWL) 
+                                (M : Interface.S Key) (MO : MapInterface Key Data M) <: IsBdlLvl MO.
+
+Include IsLvlMapKDInterface Key Data M MO.
+Import MO OP.P.
+
+Parameter Wf_in_iff : forall (m n : Lvl.t) (x : M.key) (t : t),
+  Wf m t -> M.In x (shift m n t) <-> M.In x t.
+
+Parameter shift_find_Wf : forall (k n : Lvl.t) (x : M.key) (m m' : t),
+  Key.Wf k x -> M.In x m ->
+  M.find x m = M.find x m' -> M.find x (shift k n m) = M.find x (shift k n m').
+
+Parameter shift_wf_refl : forall k n t, Wf k t -> eq (shift k n t) t.
+
+End IsBdlLvlMapKDInterface.
+
+(** ** Alternative Leveled Map Interface - [LvlK/LvlD] *)
+Module Type IsLvlFullMapKDInterface (Key : IsBdlLvlFullOTWL) (Data : IsLvlFullETWL)  
+                                    (M : Interface.S Key) (MO : MapInterface Key Data M)
+:= (IsLvlMapKDInterface Key Data M MO) <+ IsWFFull MO.
+
+(** ** Alternative Bindless Leveled Map Interface - [LvlK/LvlD] *)
+Module Type IsBdlLvlFullMapKDInterface (Key : IsBdlLvlFullOTWL) (Data : IsBdlLvlFullETWL) 
+                                       (M : Interface.S Key) (MO : MapInterface Key Data M) 
+:=  (IsBdlLvlMapKDInterface Key Data M MO) <+ IsWFFull MO.
+
+
+(** ---- *)
+
+
+(** ** Leveled Map Interface - [LevelK/ETD] *)
+Module Type IsLvlMapLVLInterface (Data : EqualityType) (M : Interface.S Level) 
+                                 (MO : MapLVLInterface Data M) <: IsLvl MO.
+
+Include IsLvlMapKInterface Level Data M MO.
+Import MO OP.P.
+
+Section specs.
+
+Variable k m n : Lvl.t.
+Variable x: M.key.
+Variable t t' : t.
+
+Parameter Wf_in_iff : Wf m t -> M.In x (shift m n t) <-> M.In x t.
+
+Parameter shift_in_new_key : M.In x (shift (new_key t) n t) <-> M.In x t.
+
+Parameter shift_find_Wf :
+  Level.Wf k x -> M.In x t ->
+  M.find x t = M.find x t' -> M.find x (shift k n t) = M.find x (shift k n t').
+
+Parameter shift_new_notin : k >= (new_key t) -> ~ M.In k (shift k n t).
+
+Parameter shift_new_refl : k >= (new_key t) -> new_key (shift k n t) = new_key t.
+
+Parameter shift_max_refl : k >= (new_key t) -> max_key (shift k n t) = max_key t.
+
+Parameter shift_max_key_gt_iff : max_key t > n <-> max_key (shift k m t) > (Level.shift k m n).
+
+Parameter shift_max_key_le : max_key t <= max_key (shift k n t).
+
+Parameter shift_new_key_le : new_key t <= new_key (shift k n t).
+
+End specs.
+
+End IsLvlMapLVLInterface.
+
+(** ** Bindless Leveled Map Interface - [LevelK/ETD] *)
+Module Type IsBdlLvlMapLVLInterface 
+  (Data : EqualityType) (M : Interface.S Level) (MO : MapLVLInterface Data M) <: IsBdlLvl MO
+:= IsLvlMapLVLInterface Data M MO <+ IsBindlessLeveledEx MO.
+
+(** ** Alter. Leveled Map Interface - [LevelK/ETD] *)
+Module Type IsLvlFullMapLVLInterface
+  (Data : EqualityType) (M : Interface.S Level) (MO : MapLVLInterface Data M)
+:= (IsLvlMapLVLInterface Data M MO) <+ IsWFFull MO.
+
+(** ** Alter. Bindless Leveled Map Interface - [LevelK/ETD] *)
+Module Type IsBdlLvlFullMapLVLInterface 
+  (Data : EqualityType) (M : Interface.S Level) (MO : MapLVLInterface Data M)
+:=  (IsBdlLvlMapLVLInterface Data M MO) <+ IsWFFull MO.
+
+(** ---- *)
+
+(** ** Leveled Map Interface - [LevelK/LvlD]  *)
+
+Module Type IsLvlMapLVLDInterface 
+  (Data : IsLvlETWL) (M : Interface.S Level) (MO : MapLVLInterface Data M) <: IsLvl MO.
+
+Include IsLvlMapKDInterface Level Data M MO.
+Import MO OP.P.
+
+Section props.
+
+Variable k m n : Lvl.t.
+Variable x : M.key.
+Variable t t' : t.
+
+Parameter Wf_in_iff : Wf m t -> M.In x (shift m n t) <-> M.In x t.
+
+Parameter shift_find_Wf :
+  Level.Wf k x -> M.In x t ->
+  M.find x t = M.find x t' -> M.find x (shift k n t) = M.find x (shift k n t').
+  
+Parameter shift_in_new_key : M.In x (shift (new_key t) n t) <-> M.In x t.
+
+Parameter shift_new_notin : k >= (new_key t) -> ~ M.In k (shift k n t).
+
+Parameter shift_new_refl : k >= (new_key t) -> new_key (shift k n t) = new_key t.
+
+Parameter shift_max_refl : k >= (new_key t) -> max_key (shift k n t) = max_key t.
+
+Parameter shift_max_key_gt_iff : max_key t > n <-> max_key (shift k m t) > (Level.shift k m n).
+
+Parameter shift_max_key_le : max_key t <= max_key (shift k n t).
+
+Parameter shift_new_key_le : new_key t <= new_key (shift k n t).
+
+End props.
+
+End IsLvlMapLVLDInterface.
+
+(** ** Bindless Leveled Map Interface - [LevelK/LvlD]  *)
+Module Type IsBdlLvlMapLVLDInterface  
+  (Data : IsBdlLvlETWL) (M : Interface.S Level) (MO : MapLVLInterface Data M) <: IsBdlLvl MO
+:= IsLvlMapLVLDInterface Data M MO <+ IsBindlessLeveledEx MO.
+
+(** ** Alter. Leveled Map Interface - [LevelK/LvlD]  *)
+Module Type IsLvlFullMapLVLDInterface
+  (Data : IsLvlFullETWL) (M : Interface.S Level) (MO : MapLVLInterface Data M)
+:= (IsLvlMapLVLDInterface Data M MO) <+ IsWFFull MO.
+
+(** ** Alter. Bindless Leveled Map Interface - [LevelK/LvlD]  *)
+Module Type IsBdlLvlFullMapLVLDInterface  
+  (Data : IsBdlLvlFullETWL) (M : Interface.S Level) (MO : MapLVLInterface Data M) 
+:=  (IsBdlLvlMapLVLDInterface Data M MO) <+ IsWFFull MO.
