theories/Map/MapLevelLvl.v
@@ -1,0 +1,209 @@
+From Coq Require Import Lia Arith.PeanoNat Classical_Prop Classes.RelationClasses.
+From MMaps Require Import MMaps.
+From DeBrLevel Require Import LevelInterface Level MapExtInterface 
+                              MapExt MapLevelInterface MapLevelK.
+
+(** * Implementation - Map - [LevelK/ETD] *)
+
+(** ** Leveled Map Implementation *)
+
+Module IsLvlMapLVL 
+  (Data : EqualityType) (M : Interface.S Level) 
+  (MO : MapLVLInterface Data M)  <: IsLvlMapLVLInterface Data M MO.
+
+Include IsLvlMapK Level Data M MO.
+Import MO OP.P.
+
+Lemma shift_new_notin (lb k : Lvl.t) (t : t) : lb >= (new_key t) -> ~ M.In lb (shift lb k t).
+Proof.
+  induction t using map_induction; intros Hgeq.
+  - rewrite shift_Empty; auto.
+    rewrite Empty_eq; auto. 
+    apply not_in_empty.
+  - unfold Add in H0; rewrite H0 in *; clear H0. 
+    rewrite shift_add.
+    rewrite new_key_add_max in Hgeq.
+    rewrite add_in_iff. 
+    intros [Heq | HIn]; subst.
+    -- unfold Level.shift in Heq.
+       destruct (Lvl.leb_spec0 lb x) as [Hle | Hnle]; lia.
+    -- apply IHt1; auto; lia.
+Qed.
+
+Lemma shift_max_refl (lb k : Lvl.t) (t : t) :
+  lb >= (new_key t) -> max_key (shift lb k t) = max_key t.
+Proof.
+  induction t using map_induction; intro Hleb.
+  - rewrite shift_Empty; auto.
+  - unfold Add in H0; rewrite H0 in *; clear H0.
+    rewrite new_key_add_max in *.
+    rewrite shift_add.
+    assert (Hle1: lb >= new_key t1) by lia.
+    apply IHt1 in Hle1.
+    do 2 rewrite max_key_add_max.
+    rewrite Hle1; f_equal.
+    rewrite Level.shift_wf_refl; auto. 
+    unfold Level.Wf.
+    assert (HIn : M.In x (M.add x e t1)).
+    { rewrite add_in_iff; now left. }
+    apply new_key_in in HIn; lia.
+Qed.
+
+Lemma shift_new_refl (lb k : Lvl.t) (t : t) :
+  lb >= (new_key t) -> new_key (shift lb k t) = new_key t.
+Proof.
+  intro Hge; repeat rewrite new_key_unfold.
+  destruct (M.is_empty t) eqn:HEmp.
+  - rewrite shift_Empty.
+    -- now rewrite HEmp.
+    -- now apply is_empty_2.
+  - destruct (M.is_empty (shift lb k t)) eqn:HEmp'.
+    -- rewrite shift_Empty in HEmp'.
+       + now rewrite HEmp in *.
+       + apply is_empty_2 in HEmp'. 
+         now rewrite <- shift_Empty_iff in HEmp'.
+    -- f_equal; now apply shift_max_refl.
+Qed.  
+
+Lemma shift_max_key_gt_iff (m n x : Lvl.t) (o : t) :
+  max_key o > x <-> max_key (shift m n o) > (Level.shift m n x).
+Proof.
+  revert x; induction o using map_induction; intro y.
+  - split; intro Hmax.
+    -- rewrite max_key_Empty in Hmax; auto; lia.
+    -- rewrite shift_Empty in Hmax; auto.
+       rewrite max_key_Empty in Hmax; auto; lia.
+  - split; intro Hmax;
+    unfold Add in H0; rewrite H0 in *; clear H0.
+    -- rewrite shift_add. 
+       rewrite max_key_add_max.
+       destruct (Lvl.leb_spec0 (max_key o1) x) as [Hle | Hgt].
+       + rewrite max_key_add_l in Hmax; auto.
+         apply (Level.shift_gt_iff m n) in Hmax; lia.
+       + rewrite max_key_add_r in Hmax by lia.
+         apply IHo1 in Hmax; lia.
+    -- rewrite shift_add in Hmax. 
+       rewrite max_key_add_max.
+       destruct (Lvl.leb_spec0 (max_key (shift m n o1)) (Level.shift m n x)) as [Hle' | Hgt'].
+       + rewrite max_key_add_l in Hmax; auto.
+         apply (Level.shift_gt_iff m n) in Hmax; lia.
+       + rewrite max_key_add_r in Hmax by lia.
+         apply IHo1 in Hmax; lia.
+Qed. 
+
+Lemma shift_max_key_le (m n : Lvl.t) (o : t) :
+  max_key o <= max_key (shift m n o).
+Proof.
+  induction o using map_induction.
+  - now rewrite shift_Empty.
+  - unfold Add in H0; rewrite H0; clear H0. 
+    rewrite shift_add.
+    do 2 rewrite max_key_add_max.
+    assert (x <= (Level.shift m n x)) by apply Level.shift_le.
+    lia.
+Qed.
+       
+Lemma shift_new_key_le (m n : Lvl.t) (o : t) :
+  new_key o <= new_key (shift m n o).
+Proof.
+  repeat rewrite new_key_unfold.
+  destruct (M.is_empty o) eqn:Hemp; try lia.
+  destruct (M.is_empty (shift m n o)) eqn:Hemp'.
+  - apply is_empty_2 in Hemp'. 
+    rewrite <- (shift_Empty_iff m n) in Hemp'.
+    apply is_empty_1 in Hemp'.
+    rewrite Hemp in Hemp'; now inversion Hemp'.
+  - assert (max_key o <= max_key (shift m n o)); try lia.
+    apply shift_max_key_le.
+Qed.
+
+Lemma Wf_in_iff (m n : Lvl.t) (x : M.key) (t : t) :
+  Wf m t -> M.In x (shift m n t) <-> M.In x t.
+Proof.
+  revert x; induction t using map_induction; intros y Hvo; split; intro HIn.
+  - rewrite shift_Empty in HIn; auto.
+  - rewrite shift_Empty; auto.
+  - unfold Add in *; rewrite H0 in *; clear H0. 
+    apply Wf_add_notin in Hvo as [Hvk Hv]; auto.
+    rewrite shift_add_notin in HIn; auto.
+    rewrite add_in_iff in *; destruct HIn as [Heq | HIn]; subst.
+    -- left; now rewrite Level.shift_wf_refl; auto.
+    -- right. rewrite <- IHt1; eauto.
+  - unfold Add in *; rewrite H0 in *; clear H0. 
+    apply Wf_add_notin in Hvo as [Hvk Hv]; auto.
+    rewrite shift_add_notin; auto.
+    rewrite add_in_iff in *; destruct HIn as [Heq | HIn]; subst.
+    -- left; now rewrite Level.shift_wf_refl; auto.
+    -- right. rewrite IHt1; eauto.
+Qed.
+
+Lemma shift_find_Wf (lb k : Lvl.t) (x : M.key) (m m' : t) :
+  Level.Wf lb x -> M.In x m ->
+  M.find x m = M.find x m' -> M.find x (shift lb k m) = M.find x (shift lb k m').
+Proof.
+  intros Hvk HIn Hfi. 
+  destruct HIn as [v HfV]; apply find_1 in HfV.
+  rewrite <- (Level.shift_wf_refl lb k x); auto.
+  now do 2 rewrite <- (shift_find lb k).
+Qed.
+
+Lemma shift_in_new_key (n : Lvl.t) (x : M.key) (t : t) :
+  M.In x (shift (new_key t) n t) <-> M.In x t.
+Proof.
+  split; intro HIn.
+  - apply shift_in_e in HIn as H.
+    destruct H as [y Heq]; subst.
+    rewrite <- shift_in_iff in HIn.
+    apply new_key_in in HIn as Hlt.
+    rewrite Level.shift_wf_refl; auto.
+  - apply new_key_in in HIn as Hlt.
+    rewrite <- (Level.shift_wf_refl (new_key t) n x); auto.
+    now rewrite <- shift_in_iff.
+Qed.
+
+End IsLvlMapLVL.
+
+(** ** Bindless Leveled Map Implementation *)
+Module IsBdlLvlMapLVL 
+  (Data : EqualityType) (M : Interface.S Level) 
+  (MO : MapLVLInterface Data M) <: IsBdlLvlMapLVLInterface Data M MO.
+
+Include IsLvlMapLVL Data M MO.
+Import MO OP.P.
+
+Lemma shift_wf_refl (lb k : Lvl.t) (t : t) : Wf lb t -> eq (shift lb k t) t.
+Proof.
+  induction t using map_induction; intro Hvt.
+  - now apply shift_Empty.
+  - unfold Add in H0; rewrite H0 in *; clear H0.
+    rewrite <- Wf_add_iff in Hvt. 
+    destruct Hvt as [Hvx Hvt].
+    rewrite shift_add.
+    rewrite IHt1; auto.
+    now rewrite Level.shift_wf_refl; auto.
+Qed.
+    
+End IsBdlLvlMapLVL.
+
+(** ---- *)
+
+(** * Make - Leveled Map [LevelK/ETD] *)
+
+Module MakeLvlMapLVL (Data : EqualityType) <: IsLvlET.
+  
+Module Raw := MMaps.OrdList.Make Level.
+Module Ext := MapETLVL Data Raw.
+Include IsLvlMapLVL Data Raw Ext.
+Include OP.P.
+
+End MakeLvlMapLVL.
+
+
+Module MakeBdlLvlMapLVL (Data : EqualityType) <: IsBdlLvlET.
+  
+Module Raw := MMaps.OrdList.Make Level.
+Module Ext := MapETLVL Data Raw.
+Include IsBdlLvlMapLVL Data Raw Ext.
+Include OP.P.
+
+End MakeBdlLvlMapLVL.
