theories/Map/Mapkit/MapExtInterface.v
@@ -1,0 +1,233 @@
+Require Import Arith.PeanoNat MSets.
+From DeBrLevel Require Import Level.
+From MMaps Require Import MMaps.
+
+(** * Interface - [MMaps] extension *)
+
+(** ** Extension of [MMaps] with new functions [Submap] and [For_all] *)
+Module Type MapInterface (Key : OrderedTypeWithLeibniz) (Data : EqualityType)  
+                                                        (M : Interface.S Key) <: EqualityType.
+
+Module OP := Facts.OrdProperties Key M.
+Import OP.P.
+
+(** *** Definitions *)
+
+Definition t : Type := M.t Data.t.
+Definition eq := @M.Equal Data.t.
+
+Parameter Submap : t -> t -> Prop. 
+Parameter For_all : (Key.t -> Data.t -> Prop) -> t -> Prop.
+
+(** *** Specifications *)
+Section specifications.
+
+Variable x : Key.t.
+Variable e e' : Data.t.
+Variable m m' m1 : t.
+
+(** **** [eq] specification *)
+
+#[export] Declare Instance eq_equiv : Equivalence eq.
+
+(** **** [Empty] specifications extension *)
+
+#[export] Declare Instance Empty_eq_iff : Proper (eq ==> iff) Empty.
+
+Parameter Empty_eq : Empty m -> eq m M.empty.
+
+Parameter notEmpty_Add : Add x e m m' -> ~ Empty m'.
+
+Parameter notEmpty_find : Empty m -> ~ (M.find x m = Some e).
+
+(** **** [is_empty] specifications extension *)
+
+Parameter is_empty_Add : Add x e m m' -> M.is_empty m' = false.
+
+Parameter is_empty_add : M.is_empty (M.add x e m) = false.
+
+(** **** [Add] specifications extension *)
+
+#[export] Declare Instance Add_eq_iff: 
+  Proper (Key.eq ==> eq ==> eq ==> iff) (fun (k : Key.t) => Add k e).
+
+(** **** [add] specifications extension *)
+
+Parameter add_shadow : eq (M.add x e (M.add x e' m)) (M.add x e m). 
+
+Parameter add_remove : M.find x m = Some e -> eq m (M.add x e (M.remove x m)).
+
+(** **** [Submap] specifications extension *)
+
+Parameter Submap_Empty_bot : Empty m -> Submap m m'.
+
+Parameter Submap_Empty : Submap m m' -> Empty m' -> Empty m.
+
+Parameter Submap_empty_bot : Submap M.empty m.
+
+Parameter Submap_Add : Submap m' m1 -> ~ M.In x m -> Add x e m m' -> Submap m m1.
+
+Parameter Submap_Add_in : Submap m' m1 -> ~ M.In x m -> Add x e m m' -> M.In x m1.
+
+Parameter Submap_Add_find : Submap m' m1 -> ~ M.In x m -> Add x e m m' ->  M.find x m1 = Some e.
+
+Parameter Submap_Add_1 : Submap m m1 ->
+                         ~ M.In x m -> M.find x m1 = Some e -> Add x e m m' -> Submap m' m1.
+
+Parameter Submap_add : Submap m m' -> Submap (M.add x e m) (M.add x e m').
+
+Parameter Submap_add_2 : ~ M.In x m -> Submap (M.add x e m) m' -> Submap m m'.
+
+Parameter Submap_add_1 : ~ M.In x m' -> Submap m m' -> Submap m (M.add x e m').
+
+Parameter Submap_in :  Submap m m' -> M.In x m -> M.In x m'.
+
+Parameter Submap_notin : Submap m m' -> ~M.In x m' -> ~M.In x m.
+
+Parameter Submap_find : Submap m m' -> M.find x m = Some e -> M.find x m' = Some e.
+
+#[export] Declare Instance Submap_refl : Reflexive Submap.
+
+#[export] Declare Instance Submap_trans : Transitive Submap.
+
+#[export] Declare Instance Submap_eq : Proper (eq ==> eq ==> iff) Submap.
+
+#[export] Declare Instance Submap_po : PreOrder Submap.
+
+(** **** [For_all] specifications *)
+
+Hypothesis P : Key.t -> Data.t -> Prop. 
+
+Parameter For_all_empty : For_all P M.empty.
+
+Parameter For_all_Empty : Empty m -> For_all P m.
+
+Parameter For_all_add : P x e /\ For_all P m -> For_all P (M.add x e m).
+
+Parameter For_all_add_notin : ~ M.In x m -> ((P x e /\ For_all P m) <-> For_all P (M.add x e m)).
+
+#[export] Declare Instance For_all_proper : Proper (eq ==> iff) (For_all P).
+
+End specifications.
+
+End MapInterface.
+
+
+(** ---- *)
+
+
+(** ** Extension of [MMaps] with new functions [max_key] and [new_key] *)
+Module Type MapLVLInterface (Data : EqualityType) 
+                                (M : Interface.S Level) <: MapInterface Level Data M.
+
+Include MapInterface Level Data M.
+Import OP.P.
+
+(** *** Definitions *)
+
+Parameter max_key : t -> nat.
+Parameter new_key : t -> nat.
+
+(** *** Specifications *)
+Section specs.
+
+Variable x : M.key.
+Variable v v' : Data.t.
+Variable m m' : t.
+
+(** **** [max_key] specifications *)
+
+#[export] Declare Instance max_key_eq : Proper (eq ==> Logic.eq) max_key.
+
+Parameter max_key_ub : x > max_key m -> for_all_dom (fun y => y <? x) m = true.
+
+Parameter max_key_Empty : Empty m -> max_key m = 0.
+
+Parameter max_key_empty : max_key M.empty = 0.
+(* begin hide *)
+(* 
+Parameter max_key_Add_spec : Add x v m m' ->
+    (max_key m' = x /\ max_key m <= x) \/ (max_key m' = max_key m /\ max_key m > x). *)
+(* end hide *)
+
+Parameter max_key_Add_l : Add x v m m' ->  max_key m <= x -> max_key m' = x.
+
+Parameter max_key_Add_r : Add x v m m' ->  max_key m > x -> max_key m' = max_key m.
+
+Parameter max_key_Add_max : Add x v m m' -> max_key m' = max x (max_key m).
+(* begin hide *)
+(* Parameter max_key_add_spec :
+  ~M.In x m -> (max_key (M.add x v m) = x /\ max_key m <= x) \/ 
+               (max_key (M.add x v m) = max_key m /\ max_key m > x). *)
+(* end hide *)
+
+Parameter max_key_add_l : max_key m <= x -> max_key (M.add x v m) = x.
+
+Parameter max_key_add_r : max_key m > x -> max_key (M.add x v m) = max_key m.
+
+Parameter max_key_add_in : M.In x m -> (max_key (M.add x v m)) = (max_key m).
+
+Parameter max_key_add_iff : max_key m = max_key m' -> 
+                            max_key (M.add x v m) = max_key (M.add x v' m').
+
+Parameter max_key_add_max_key : max_key (M.add (S (max_key m)) v m) = S (max_key m).
+
+Parameter max_key_add_max : max_key (M.add x v m) = max x (max_key m).
+
+Parameter max_key_notin : x > max_key m -> ~ M.In x m.
+
+Parameter max_key_in : M.In x m -> x <= (max_key m).
+
+Parameter max_key_Submap : Submap m m' -> max_key m <= max_key m'.
+
+(** **** [new_key] specifications *)
+
+#[export] Declare Instance new_key_eq : Proper (eq ==> Logic.eq) new_key.
+
+Parameter new_key_geq_max_key : new_key m >= max_key m. 
+
+Parameter new_key_unfold : new_key m = if M.is_empty m then 0 else S (max_key m).
+
+Parameter new_key_Empty : Empty m -> new_key m = 0.
+
+Parameter new_key_empty : new_key M.empty = 0.
+(* begin hide *)
+(* 
+Parameter new_key_Add_spec : ~M.In x m -> Add x v m m' ->
+    (new_key m' = S x /\ new_key m <= S x) \/ (new_key m' = new_key m /\ new_key m > S x).
+*)
+(* end hide *)
+
+Parameter new_key_Add_l : Add x v m m' ->  new_key m <= S x -> new_key m' = S x.
+
+Parameter new_key_Add_r : Add x v m m' ->  new_key m > S x -> new_key m' = new_key m.
+
+Parameter new_key_Add_max : Add x v m m' -> new_key m' = max (S x) (new_key m).
+(* begin hide *)
+(* Parameter new_key_add_spec :
+  ~M.In x m -> (new_key (M.add x v m) = S x /\ new_key m <= S x) \/ 
+               (new_key (M.add x v m) = new_key m /\ new_key m > S x).*)
+(* end hide *)
+
+Parameter new_key_add_max : new_key (M.add x v m) = max (S x) (new_key m).
+
+Parameter new_key_add_l : new_key m <= S x -> new_key (M.add x v m) = S x.
+
+Parameter new_key_add_r : new_key m > S x -> new_key (M.add x v m) = new_key m.
+
+Parameter new_key_add_in : M.In x m -> (new_key (M.add x v m)) = (new_key m).
+
+Parameter new_key_add_new_key : new_key (M.add (new_key m) v m) = S (new_key m).
+
+Parameter new_key_notin : x >= new_key m -> ~ M.In x m.
+
+Parameter new_key_in : M.In x m -> x < new_key m.
+
+Parameter new_key_Submap : Submap m m' -> new_key m <= new_key m'.
+
+Parameter new_key_Submap_add : Submap m m' -> 
+                               Submap m (M.add (S (new_key m')) v (M.add (new_key m') v' m')).
+
+End specs.
+
+End MapLVLInterface.
